POPL24

coq/theories/logical_sn.v
@@ -1,6 +1,8 @@
+(* This file presents the strong normalization of the logical level.  *)
+
 From mathcomp Require Import ssreflect ssrbool eqtype ssrnat seq.
 From Coq Require Import ssrfun Classical Utf8.
-Require Export AutosubstSsr ARS mltt_subst sta_subst.
+Require Export AutosubstSsr ARS mltt_subst logical_subst.
 
 Set Implicit Arguments.
 Unset Strict Implicit.
@@ -11,41 +13,42 @@ Section Model.
 Declare Scope model_scope.
 Open Scope model_scope.
 
-Fixpoint interp (m : tll_ast.term) : mltt_ast.term :=
+(* Modeling logical TLL in MLTT. *)
+Fixpoint model (m : tll_ast.term) : mltt_ast.term :=
   match m with
   | tll_ast.Var x => mltt_ast.Var x
   | tll_ast.Sort _ => mltt_ast.Ty
-  | tll_ast.Pi0 A B _ => mltt_ast.Pi (interp A) (interp B)
-  | tll_ast.Pi1 A B _ => mltt_ast.Pi (interp A) (interp B)
-  | tll_ast.Lam0 A m _ => mltt_ast.Lam (interp A) (interp m)
-  | tll_ast.Lam1 A m _ => mltt_ast.Lam (interp A) (interp m)
-  | tll_ast.App m n => mltt_ast.App (interp m) (interp n)
-  | tll_ast.Sig0 A B _ => mltt_ast.Sig (interp A) (interp B)
-  | tll_ast.Sig1 A B _ => mltt_ast.Sig (interp A) (interp B)
-  | tll_ast.Pair0 m n _ => mltt_ast.DPair (interp m) (interp n)
-  | tll_ast.Pair1 m n _ => mltt_ast.DPair (interp m) (interp n)
-  | tll_ast.LetIn A m n => mltt_ast.LetIn (interp A) (interp m) (interp n)
-  | tll_ast.With A B _ => mltt_ast.Tuple (interp A) (interp B)
-  | tll_ast.APair m n _ => mltt_ast.Pair (interp m) (interp n)
-  | tll_ast.Fst m => mltt_ast.Fst (interp m)
-  | tll_ast.Snd m => mltt_ast.Snd (interp m)
-  | tll_ast.Id A m n => mltt_ast.Id (interp A) (interp m) (interp n)
-  | tll_ast.Refl m => mltt_ast.Refl (interp m)
-  | tll_ast.Rw A H P => mltt_ast.Rw (interp A) (interp H) (interp P)
+  | tll_ast.Pi0 A B _ => mltt_ast.Pi (model A) (model B)
+  | tll_ast.Pi1 A B _ => mltt_ast.Pi (model A) (model B)
+  | tll_ast.Lam0 A m _ => mltt_ast.Lam (model A) (model m)
+  | tll_ast.Lam1 A m _ => mltt_ast.Lam (model A) (model m)
+  | tll_ast.App m n => mltt_ast.App (model m) (model n)
+  | tll_ast.Sig0 A B _ => mltt_ast.Sig (model A) (model B)
+  | tll_ast.Sig1 A B _ => mltt_ast.Sig (model A) (model B)
+  | tll_ast.Pair0 m n _ => mltt_ast.DPair (model m) (model n)
+  | tll_ast.Pair1 m n _ => mltt_ast.DPair (model m) (model n)
+  | tll_ast.LetIn A m n => mltt_ast.LetIn (model A) (model m) (model n)
+  | tll_ast.With A B _ => mltt_ast.Tuple (model A) (model B)
+  | tll_ast.APair m n _ => mltt_ast.Pair (model m) (model n)
+  | tll_ast.Fst m => mltt_ast.Fst (model m)
+  | tll_ast.Snd m => mltt_ast.Snd (model m)
+  | tll_ast.Id A m n => mltt_ast.Id (model A) (model m) (model n)
+  | tll_ast.Refl m => mltt_ast.Refl (model m)
+  | tll_ast.Rw A H P => mltt_ast.Rw (model A) (model H) (model P)
   | tll_ast.Box => mltt_ast.Ty
   | tll_ast.Ptr _ => mltt_ast.Ty
   end.
 
-Fixpoint interp_ctx (Γ : sta_ctx) : mltt_ctx :=
+Fixpoint model_ctx (Γ : logical_ctx) : mltt_ctx :=
   match Γ with
   | nil => nil
-  | A :: Γ => interp A :: interp_ctx Γ
+  | A :: Γ => model A :: model_ctx Γ
   end.
 
-Notation "[| m |]" := (interp m).
-Notation "[[ Γ ]]" := (interp_ctx Γ).
+Notation "[| m |]" := (model m).
+Notation "[[ Γ ]]" := (model_ctx Γ).
 
-Lemma interp_ren_com m ξ :
+Lemma model_ren_com m ξ :
   [| m |].[ren ξ] = [| m.[ren ξ] |].
 Proof with eauto.
   elim: m ξ=>//=...
@@ -82,23 +85,23 @@ Proof with eauto.
     rewrite ihA. rewrite ihH. rewrite ihP... }
 Qed.
 
-Definition interp_subst
+Definition model_subst
   (σ : var -> tll_ast.term)
   (τ : var -> mltt_ast.term) : Prop := forall x, [|σ x|] = τ x.
 
-Lemma interp_subst_up σ τ :
-  interp_subst σ τ -> interp_subst (up σ) (up τ).
+Lemma model_subst_up σ τ :
+  model_subst σ τ -> model_subst (up σ) (up τ).
 Proof with eauto.
-  unfold interp_subst.
+  unfold model_subst.
   move=>h x.  elim: x σ τ h...
   move=>n ih σ τ h. asimpl.
-  rewrite<-interp_ren_com.
+  rewrite<-model_ren_com.
   rewrite h...
 Qed.
 
-Lemma interp_subst_com m σ τ :
-  interp_subst σ τ -> [| m.[σ] |] = [| m |].[τ].
-Proof with eauto using interp_subst_up.
+Lemma model_subst_com m σ τ :
+  model_subst σ τ -> [| m.[σ] |] = [| m |].[τ].
+Proof with eauto using model_subst_up.
   elim: m σ τ=>//=.
   { move=>A ihA B ihB _ σ τ h.
     rewrite (ihA _ τ)...
@@ -152,102 +155,104 @@ Proof with eauto using interp_subst_up.
     rewrite (ihP _ τ)... }
 Qed.
 
-Lemma interp_step m n : sta_step m n -> mltt_step [|m|] [|n|].
+(* Lemma 2 (Logical Reduction Model) *)
+Lemma model_step m n : logical_step m n -> mltt_step [|m|] [|n|].
 Proof with eauto using mltt_step.
   elim=>//={m n}...
   { move=>A m n _.
-    erewrite interp_subst_com.
+    erewrite model_subst_com.
     constructor. move=>x. destruct x=>//. }
   { move=>A m n _.
-    erewrite interp_subst_com.
+    erewrite model_subst_com.
     constructor. move=>x. destruct x=>//. }
   { move=>A m1 m2 n _.
-    erewrite interp_subst_com.
+    erewrite model_subst_com.
     constructor. move=>x.
     destruct x=>//.
     destruct x=>//. }
   { move=>A m1 m2 n _.
-    erewrite interp_subst_com.
+    erewrite model_subst_com.
     constructor. move=>x.
     destruct x=>//.
     destruct x=>//. }
 Qed.
 
-Lemma interp_red m n : sta_red m n -> mltt_red [|m|] [|n|].
+Lemma model_red m n : logical_red m n -> mltt_red [|m|] [|n|].
 Proof with eauto using mltt_step, star.
   elim=>{n}...
   move=>y z rd1 rd2 st.
   apply: star_trans...
   apply: star1.
-  apply: interp_step...
+  apply: model_step...
 Qed.
 
-Lemma interp_conv m n :
-  conv sta_step m n -> conv mltt_step [|m|] [|n|].
+Lemma model_conv m n :
+  conv logical_step m n -> conv mltt_step [|m|] [|n|].
 Proof with eauto using mltt_step, conv.
   elim=>{n}...
   { move=>y z eq1 eq2 st.
     apply: conv_trans...
     apply: conv1.
-    apply: interp_step... }
+    apply: model_step... }
   { move=>y z eq1 eq2 st.
     apply: conv_trans...
     apply: conv_sym.
     apply: conv1.
-    apply: interp_step... }
+    apply: model_step... }
 Qed.
 
-Lemma interp_has Γ x A :
-  sta_has Γ x A -> mltt_has [[Γ]] x [|A|].
+Lemma model_has Γ x A :
+  logical_has Γ x A -> mltt_has [[Γ]] x [|A|].
 Proof with eauto using mltt_has.
   elim=>//={Γ x A}.
-  { move=>Γ A. rewrite<-interp_ren_com... }
-  { move=>Γ A B x shs ih. rewrite<-interp_ren_com... }
+  { move=>Γ A. rewrite<-model_ren_com... }
+  { move=>Γ A B x shs ih. rewrite<-model_ren_com... }
 Qed.
 
-Theorem sta_mltt_interp Γ m A :
-  sta_type Γ m A -> mltt_type [[Γ]] [|m|] [|A|].
+(* Logical Type Model *)
+Theorem logical_mltt_model Γ m A :
+  logical_type Γ m A -> mltt_type [[Γ]] [|m|] [|A|].
 Proof with eauto using mltt_type, mltt_wf.
-  move:Γ m A. apply: (@sta_type_mut _ (fun Γ wf=> mltt_wf [[Γ]])); simpl...
+  move:Γ m A. apply: (@logical_type_mut _ (fun Γ wf=> mltt_wf [[Γ]])); simpl...
   { move=>Γ x A wf1 wf2 shs.
     constructor...
-    apply: interp_has... }
+    apply: model_has... }
   { move=>Γ A B m n s tym ihm tyn ihn.
-    erewrite interp_subst_com...
+    erewrite model_subst_com...
     move=>x. destruct x=>//. }
   { move=>Γ A B m n s tym ihm tyn ihn.
-    erewrite interp_subst_com...
+    erewrite model_subst_com...
     move=>x. destruct x=>//. }
   { move=>Γ A B m n t _ _ tym ihm tyn ihn.
     constructor...
-    erewrite<-interp_subst_com...
+    erewrite<-model_subst_com...
     move=>x. destruct x=>//. }
   { move=>Γ A B m n t _ _ tym ihm tyn ihn.
     constructor...
-    erewrite<-interp_subst_com...
+    erewrite<-model_subst_com...
     move=>x. destruct x=>//. }
   { move=>Γ A B C m n s t tyC ihC tym ihm tyn ihn.
-    erewrite interp_subst_com...
+    erewrite model_subst_com...
     econstructor...
-    erewrite<-interp_subst_com...
+    erewrite<-model_subst_com...
     move=>x. destruct x=>//.
     move=>x. destruct x=>//. }
   { move=>Γ A B C m n s t tyC ihC tym ihm tyn ihn.
-    erewrite interp_subst_com...
+    erewrite model_subst_com...
     econstructor...
-    erewrite<-interp_subst_com...
+    erewrite<-model_subst_com...
     move=>x. destruct x=>//.
     move=>x. destruct x=>//. }
   { move=>Γ A B H P m n s tyB ihB tyH ihH tyP ihP.
-    erewrite interp_subst_com...
+    erewrite model_subst_com...
     apply: mltt_rw...
-    rewrite!interp_ren_com...
-    erewrite<-interp_subst_com...
+    rewrite!model_ren_com...
+    erewrite<-model_subst_com...
     move=>x. destruct x=>//=. destruct x=>//=.
     move=>x. destruct x=>//=. destruct x=>//=. }
   { move=>Γ A B m s eq tym ihm tyB ihB.
     apply: mltt_conv.
-    apply: interp_conv...
+    apply: model_conv...
     apply: ihm.
     apply: ihB. }
 Qed.
@@ -255,11 +260,11 @@ Qed.
 CoInductive nn T (Rel : T -> T -> Prop) : T -> Prop :=
 | nnI m m' : Rel m m' -> nn Rel m' -> nn Rel m.
 
-CoFixpoint interp_nn m : (nn sta_step m) -> nn mltt_step [|m|].
+CoFixpoint model_nn m : (nn logical_step m) -> nn mltt_step [|m|].
 Proof with eauto.
   move=>h. inv h.
-  move/interp_step in H.
-  move/interp_nn in H0.
+  move/model_step in H.
+  move/model_nn in H0.
   econstructor...
 Qed.
 
@@ -293,14 +298,15 @@ Proof with eauto using nn.
   firstorder...
 Qed.
 
-Theorem sta_sn Γ m A : sta_type Γ m A -> sn sta_step m.
+(* Theorem 5 (Logical Strong Normalization) *)
+Theorem logical_sn Γ m A : logical_type Γ m A -> sn logical_step m.
 Proof with eauto.
-  move=>/sta_mltt_interp ty.
+  move=>/logical_mltt_model ty.
   have h1:=mltt_sn ty.
-  have[h2|h2]:=classic (nn sta_step m).
-  { move/interp_nn in h2.
+  have[h2|h2]:=classic (nn logical_step m).
+  { move/model_nn in h2.
     exfalso. apply: nn_sn_false... }
-  { have[//|h3]:=classic (sn sta_step m).
+  { have[//|h3]:=classic (sn logical_step m).
     exfalso. apply: h2. apply: not_sn_nn... }
 Qed.
 
