coq/theories/logical_subst.v
@@ -1,6 +1,8 @@
+(* This files presents the substitution lemma for the logical level. *)
+
 From mathcomp Require Import ssreflect ssrbool eqtype ssrnat seq.
 From Coq Require Import ssrfun Classical Utf8.
-Require Export AutosubstSsr ARS sta_weak.
+Require Export AutosubstSsr ARS logical_weak.
 
 Set Implicit Arguments.
 Unset Strict Implicit.
@@ -8,52 +10,53 @@ Unset Printing Implicit Defensive.
 
 Reserved Notation "Γ1 ⊢ σ ⊣ Γ2" (at level 50, σ, Γ2 at next level).
 
-Inductive sta_agree_subst :
-  sta_ctx -> (var -> term) -> sta_ctx -> Prop :=
-| sta_agree_subst_nil σ :
+(* Relation to strengthen induction for simultaneous substitution. *)
+Inductive logical_agree_subst :
+  logical_ctx -> (var -> term) -> logical_ctx -> Prop :=
+| logical_agree_subst_nil σ :
   nil ⊢ σ ⊣ nil
-| sta_agree_subst_ty Γ1 σ Γ2 A s :
+| logical_agree_subst_ty Γ1 σ Γ2 A s :
   Γ1 ⊢ σ ⊣ Γ2 ->
   Γ2 ⊢ A : Sort s ->
   (A.[σ] :: Γ1) ⊢ up σ ⊣ (A :: Γ2)
-| sta_agree_subst_wk Γ1 σ Γ2 n A :
+| logical_agree_subst_wk Γ1 σ Γ2 n A :
   Γ1 ⊢ σ ⊣ Γ2 ->
   Γ1 ⊢ n : A.[σ] ->
   Γ1 ⊢ n .: σ ⊣ (A :: Γ2)
-| sta_agree_subst_conv Γ1 σ Γ2 A B s :
+| logical_agree_subst_conv Γ1 σ Γ2 A B s :
   A === B ->
   Γ1 ⊢ B.[ren (+1)].[σ] : Sort s ->
   Γ2 ⊢ B : Sort s ->
   Γ1 ⊢ σ ⊣ (A :: Γ2) ->
   Γ1 ⊢ σ ⊣ (B :: Γ2)
-where "Γ1 ⊢ σ ⊣ Γ2" := (sta_agree_subst Γ1 σ Γ2).
+where "Γ1 ⊢ σ ⊣ Γ2" := (logical_agree_subst Γ1 σ Γ2).
 
-Lemma sta_agree_subst_refl Γ : sta_wf Γ -> Γ ⊢ ids ⊣ Γ.
-Proof with eauto using sta_agree_subst.
+Lemma logical_agree_subst_refl Γ : logical_wf Γ -> Γ ⊢ ids ⊣ Γ.
+Proof with eauto using logical_agree_subst.
   elim=>{Γ}...
   move=>Γ A s wf agr tyA.
   have: (A.[ids] :: Γ) ⊢ up ids ⊣ (A :: Γ)...
   by asimpl...
 Qed.
-#[global] Hint Resolve sta_agree_subst_refl.
+#[global] Hint Resolve logical_agree_subst_refl.
 
-Lemma sta_agree_subst_has Γ1 σ Γ2 x A :
-  Γ1 ⊢ σ ⊣ Γ2 -> sta_wf Γ1 -> sta_has Γ2 x A -> Γ1 ⊢ σ x : A.[σ].
-Proof with eauto using sta_agree_subst.
+Lemma logical_agree_subst_has Γ1 σ Γ2 x A :
+  Γ1 ⊢ σ ⊣ Γ2 -> logical_wf Γ1 -> logical_has Γ2 x A -> Γ1 ⊢ σ x : A.[σ].
+Proof with eauto using logical_agree_subst.
   move=>agr. elim: agr x A=>{Γ1 σ Γ2}.
   { move=>σ x A wf hs. inv hs. }
   { move=>Γ1 σ Γ2 A s agr ih tyA x B wf hs.
     inv hs; asimpl.
     replace A.[σ >> ren (+1)] with A.[σ].[ren (+1)] by autosubst.
-    apply: sta_var...
+    apply: logical_var...
     constructor.
     replace A0.[σ >> ren (+1)] with A0.[σ].[ren (+1)] by autosubst.
-    inv wf. apply: sta_eweaken... }
+    inv wf. apply: logical_eweaken... }
   { move=>Γ1 σ Γ2 n A agr ih tyn x B wf hs. inv hs; asimpl... }
   { move=>Γ1 σ Γ2 A B s eq tyB1 tyB2 agr ih x C wf hs. inv hs.
-    { apply: sta_conv.
-      apply: sta_conv_subst.
-      apply: sta_conv_subst.
+    { apply: logical_conv.
+      apply: logical_conv_subst.
+      apply: logical_conv_subst.
       apply: eq.
       apply: ih...
       constructor.
@@ -62,54 +65,55 @@ Proof with eauto using sta_agree_subst.
       constructor... } }
 Qed.
 
-Lemma sta_agree_subst_wf_nil Γ1 σ : Γ1 ⊢ σ ⊣ nil -> sta_wf Γ1.
-Proof with eauto using sta_wf.
+Lemma logical_agree_subst_wf_nil Γ1 σ : Γ1 ⊢ σ ⊣ nil -> logical_wf Γ1.
+Proof with eauto using logical_wf.
   move e:(nil)=>Γ2 agr. elim: agr e=>//{Γ1 Γ2 σ}...
 Qed.
 
-Lemma sta_agree_subst_wf_cons Γ1 Γ2 A s σ :
-  Γ1 ⊢ σ ⊣ (A :: Γ2) -> sta_wf Γ2 ->
-  (∀ Γ1 σ, Γ1 ⊢ σ ⊣ Γ2 → sta_wf Γ1) ->
+Lemma logical_agree_subst_wf_cons Γ1 Γ2 A s σ :
+  Γ1 ⊢ σ ⊣ (A :: Γ2) -> logical_wf Γ2 ->
+  (∀ Γ1 σ, Γ1 ⊢ σ ⊣ Γ2 → logical_wf Γ1) ->
   (∀ Γ1 σ, Γ1 ⊢ σ ⊣ Γ2 → Γ1 ⊢ A.[σ] : Sort s) ->
-  sta_wf Γ1.
-Proof with eauto using sta_wf.
+  logical_wf Γ1.
+Proof with eauto using logical_wf.
   move e:(A :: Γ2)=>Γ0 agr. elim: agr Γ2 A s e=>//{Γ0 Γ1 σ}...
   move=>Γ1 σ Γ2 A s agr ih tyA Γ0 A0 s0 [e1 e2] wf h1 h2; subst.
-  apply: sta_wf_cons...
+  apply: logical_wf_cons...
 Qed.
 
-Lemma sta_substitution Γ1 Γ2 m A σ :
+(* Simultaneous substitution lemma. *)
+Lemma logical_substitution Γ1 Γ2 m A σ :
   Γ2 ⊢ m : A -> Γ1 ⊢ σ ⊣ Γ2 -> Γ1 ⊢ m.[σ] : A.[σ].
-Proof with eauto using sta_agree_subst, sta_type.
+Proof with eauto using logical_agree_subst, logical_type.
   move=>ty. move: Γ2 m A ty Γ1 σ.
-  apply: (@sta_type_mut _ (fun Γ2 wf => forall Γ1 σ, Γ1 ⊢ σ ⊣ Γ2 -> sta_wf Γ1))...
+  apply: (@logical_type_mut _ (fun Γ2 wf => forall Γ1 σ, Γ1 ⊢ σ ⊣ Γ2 -> logical_wf Γ1))...
   { move=>Γ2 x A wf h hs Γ1 σ agr. asimpl.
-    apply: sta_agree_subst_has... }
+    apply: logical_agree_subst_has... }
   { move=>Γ2 A B m s tym ihm Γ1 σ agr. asimpl.
-    have wf:=sta_type_wf tym. inv wf.
-    apply: sta_lam0... }
+    have wf:=logical_type_wf tym. inv wf.
+    apply: logical_lam0... }
   { move=>Γ2 A B m s tym ihm Γ1 σ agr. asimpl.
-    have wf:=sta_type_wf tym. inv wf.
-    apply: sta_lam1... }
+    have wf:=logical_type_wf tym. inv wf.
+    apply: logical_lam1... }
   { move=>Γ2 A B m n s tym ihm tyn ihn Γ1 σ agr. asimpl.
     replace B.[n.[σ] .: σ] with B.[up σ].[n.[σ]/] by autosubst.
     have{}ihm:=ihm _ _ agr.
     have{}ihn:=ihn _ _ agr.
-    apply: sta_app0.
+    apply: logical_app0.
     asimpl in ihm...
     asimpl in ihn... }
   { move=>Γ2 A B m n s tym ihm tyn ihn Γ1 σ agr. asimpl.
     replace B.[n.[σ] .: σ] with B.[up σ].[n.[σ]/] by autosubst.
     have{}ihm:=ihm _ _ agr.
     have{}ihn:=ihn _ _ agr.
-    apply: sta_app1.
+    apply: logical_app1.
     asimpl in ihm...
     asimpl in ihn... }
   { move=>Γ A B m n t tyS ihS tym ihm tyn ihn Γ1 σ agr. asimpl.
     have{}ihS:=ihS _ _ agr.
     have{}ihm:=ihm _ _ agr.
     have{}ihn:=ihn _ _ agr.
-    apply: sta_pair0.
+    apply: logical_pair0.
     asimpl in ihS...
     asimpl in ihm...
     asimpl in ihn...
@@ -118,42 +122,42 @@ Proof with eauto using sta_agree_subst, sta_type.
     have{}ihS:=ihS _ _ agr.
     have{}ihm:=ihm _ _ agr.
     have{}ihn:=ihn _ _ agr.
-    apply: sta_pair1.
+    apply: logical_pair1.
     asimpl in ihS...
     asimpl in ihm...
     asimpl in ihn...
     by autosubst. }
   { move=>Γ A B C m n s t tyC ihC tym ihm tyn ihn Γ1 σ agr. asimpl.
     replace C.[m.[σ] .: σ] with C.[up σ].[m.[σ]/] by autosubst.
-    have wf:=sta_type_wf tyC. inv wf.
-    have wf:=sta_type_wf tyn. inv wf. inv H3.
-    have{}ihC:=ihC _ _ (sta_agree_subst_ty agr H2).
+    have wf:=logical_type_wf tyC. inv wf.
+    have wf:=logical_type_wf tyn. inv wf. inv H3.
+    have{}ihC:=ihC _ _ (logical_agree_subst_ty agr H2).
     have{}ihm:=ihm _ _ agr.
-    have{}ihn:=ihn _ _ (sta_agree_subst_ty (sta_agree_subst_ty agr H6) H4).
-    apply: sta_letin0.
+    have{}ihn:=ihn _ _ (logical_agree_subst_ty (logical_agree_subst_ty agr H6) H4).
+    apply: logical_letin0.
     asimpl in ihC...
     asimpl in ihm...
     asimpl in ihn...
     by asimpl. }
   { move=>Γ A B C m n s t tyC ihC tym ihm tyn ihn Γ1 σ agr. asimpl.
     replace C.[m.[σ] .: σ] with C.[up σ].[m.[σ]/] by autosubst.
-    have wf:=sta_type_wf tyC. inv wf.
-    have wf:=sta_type_wf tyn. inv wf. inv H3.
-    have{}ihC:=ihC _ _ (sta_agree_subst_ty agr H2).
+    have wf:=logical_type_wf tyC. inv wf.
+    have wf:=logical_type_wf tyn. inv wf. inv H3.
+    have{}ihC:=ihC _ _ (logical_agree_subst_ty agr H2).
     have{}ihm:=ihm _ _ agr.
-    have{}ihn:=ihn _ _ (sta_agree_subst_ty (sta_agree_subst_ty agr H6) H4).
-    apply: sta_letin1.
+    have{}ihn:=ihn _ _ (logical_agree_subst_ty (logical_agree_subst_ty agr H6) H4).
+    apply: logical_letin1.
     asimpl in ihC...
     asimpl in ihm...
     asimpl in ihn...
     by asimpl. }
   { move=>Γ2 A B H P m n s tyB ihB tyH ihH tyP ihP Γ1 σ agr. asimpl.
     replace B.[P.[σ] .: n.[σ] .: σ] with B.[upn 2 σ].[P.[σ],n.[σ]/] by autosubst.
-    have wf:=sta_type_wf tyB. inv wf. inv H2.
-    have{}ihB:=ihB _ _ (sta_agree_subst_ty (sta_agree_subst_ty agr H5) H3).
+    have wf:=logical_type_wf tyB. inv wf. inv H2.
+    have{}ihB:=ihB _ _ (logical_agree_subst_ty (logical_agree_subst_ty agr H5) H3).
     have{}ihH:=ihH _ _ agr.
     have{}ihP:=ihP _ _ agr.
-    apply: sta_rw.
+    apply: logical_rw.
     asimpl in ihB.
     replace A.[σ >> ren (+1)] with A.[σ].[ren (+1)] in ihB by autosubst.
     replace m.[σ >> ren (+1)] with m.[σ].[ren (+1)] in ihB by autosubst.
@@ -161,44 +165,47 @@ Proof with eauto using sta_agree_subst, sta_type.
     asimpl. asimpl in ihH...
     asimpl in ihP... }
   { move=>Γ2 A B m s eq tym ihm tyB ihB Γ1 σ agr.
-    apply: sta_conv.
-    apply: sta_conv_subst.
+    apply: logical_conv.
+    apply: logical_conv_subst.
     apply: eq.
     apply: ihm...
     apply: ihB... }
   { move=>Γ1 σ agr.
-    apply: sta_agree_subst_wf_nil... }
+    apply: logical_agree_subst_wf_nil... }
   { move=>Γ A s wf ih tyA h Γ1 σ agr.
-    apply: sta_agree_subst_wf_cons... }
+    apply: logical_agree_subst_wf_cons... }
 Qed.
 
-Lemma sta_subst Γ m n A B :
+(* Single variable substitution lemma. *)
+Lemma logical_subst Γ m n A B :
   (A :: Γ) ⊢ m : B -> Γ ⊢ n : A -> Γ ⊢ m.[n/] : B.[n/].
-Proof with eauto using sta_agree_subst_refl.
+Proof with eauto using logical_agree_subst_refl.
   move=>tym tyn.
-  apply: sta_substitution...
-  apply: sta_agree_subst_wk...
+  apply: logical_substitution...
+  apply: logical_agree_subst_wk...
   by asimpl.
 Qed.
 
-Lemma sta_esubst Γ m m' n A B B' :
+(* Alternative statement more suitable for certain Coq tactics *)
+Lemma logical_esubst Γ m m' n A B B' :
   m' = m.[n/] ->
   B' = B.[n/] ->
   (A :: Γ) ⊢ m : B -> Γ ⊢ n : A -> Γ ⊢ m' : B'.
 Proof.
-  move=>*; subst. apply: sta_subst; eauto.
+  move=>*; subst. apply: logical_subst; eauto.
 Qed.
 
-Lemma sta_ctx_conv Γ m A B C s :
+(* Context conversion lemma. *)
+Lemma logical_ctx_conv Γ m A B C s :
   B === A ->
   Γ ⊢ B : Sort s -> (A :: Γ) ⊢ m : C -> (B :: Γ) ⊢ m : C.
-Proof with eauto using sta_wf, sta_agree_subst_refl.
+Proof with eauto using logical_wf, logical_agree_subst_refl.
   move=>eq tyB tym.
-  have wf:=sta_type_wf tym. inv wf.
+  have wf:=logical_type_wf tym. inv wf.
   have:(B :: Γ) ⊢ m.[ids] : C.[ids].
-  apply: sta_substitution...
-  apply: sta_agree_subst_conv...
-  apply: sta_eweaken...
+  apply: logical_substitution...
+  apply: logical_agree_subst_conv...
+  apply: logical_eweaken...
   asimpl...
   asimpl...
   asimpl...
