coq/theories/program_weak.v
@@ -1,58 +1,61 @@
+(* This file presents the weakening lemmas for the program level. *)
+
 From mathcomp Require Import ssreflect ssrbool eqtype ssrnat seq.
 From Coq Require Import ssrfun Classical Utf8.
-Require Export AutosubstSsr ARS sta_weak dyn_type.
+Require Export AutosubstSsr ARS logical_weak program_type.
 
 Set Implicit Arguments.
 Unset Strict Implicit.
 Unset Printing Implicit Defensive.
 
-Inductive dyn_agree_ren : (var -> var) ->
-  sta_ctx -> dyn_ctx -> sta_ctx -> dyn_ctx -> Prop :=
-| dyn_agree_ren_nil ξ :
-  dyn_agree_ren ξ nil nil nil nil
-| dyn_agree_ren_ty Γ Γ' Δ Δ' ξ m s :
+(* Relation to strengthen induction for generalized renaming lemma. *)
+Inductive program_agree_ren : (var -> var) ->
+  logical_ctx -> program_ctx -> logical_ctx -> program_ctx -> Prop :=
+| program_agree_ren_nil ξ :
+  program_agree_ren ξ nil nil nil nil
+| program_agree_ren_ty Γ Γ' Δ Δ' ξ m s :
   Γ ⊢ m : Sort s ->
-  dyn_agree_ren ξ Γ Δ Γ' Δ' ->
-  dyn_agree_ren (upren ξ)
+  program_agree_ren ξ Γ Δ Γ' Δ' ->
+  program_agree_ren (upren ξ)
     (m :: Γ) (m :{s} Δ) (m.[ren ξ] :: Γ') (m.[ren ξ] :{s} Δ')
-| dyn_agree_ren_n Γ Γ' Δ Δ' ξ m s :
+| program_agree_ren_n Γ Γ' Δ Δ' ξ m s :
   Γ ⊢ m : Sort s ->
-  dyn_agree_ren ξ Γ Δ Γ' Δ' ->
-  dyn_agree_ren (upren ξ)
+  program_agree_ren ξ Γ Δ Γ' Δ' ->
+  program_agree_ren (upren ξ)
     (m :: Γ) (_: Δ) (m.[ren ξ] :: Γ') (_: Δ')
-| dyn_agree_ren_wkU Γ Γ' Δ Δ' ξ m :
+| program_agree_ren_wkU Γ Γ' Δ Δ' ξ m :
   Γ' ⊢ m : Sort U ->
-  dyn_agree_ren ξ Γ Δ Γ' Δ' ->
-  dyn_agree_ren (ξ >>> (+1)) Γ Δ (m :: Γ') (m :U Δ')
-| dyn_agree_ren_wkN Γ Γ' Δ Δ' ξ m s :
+  program_agree_ren ξ Γ Δ Γ' Δ' ->
+  program_agree_ren (ξ >>> (+1)) Γ Δ (m :: Γ') (m :U Δ')
+| program_agree_ren_wkN Γ Γ' Δ Δ' ξ m s :
   Γ' ⊢ m : Sort s ->
-  dyn_agree_ren ξ Γ Δ Γ' Δ' ->
-  dyn_agree_ren (ξ >>> (+1)) Γ Δ (m :: Γ') (_: Δ').
+  program_agree_ren ξ Γ Δ Γ' Δ' ->
+  program_agree_ren (ξ >>> (+1)) Γ Δ (m :: Γ') (_: Δ').
 
-Lemma dyn_sta_agree_ren Γ Γ' Δ Δ' ξ :
-  dyn_agree_ren ξ Γ Δ Γ' Δ' -> sta_agree_ren ξ Γ Γ'.
-Proof with eauto using sta_agree_ren.
+Lemma program_logical_agree_ren Γ Γ' Δ Δ' ξ :
+  program_agree_ren ξ Γ Δ Γ' Δ' -> logical_agree_ren ξ Γ Γ'.
+Proof with eauto using logical_agree_ren.
   elim=>{Γ Γ' Δ Δ' ξ}...
 Qed.
 
-Lemma dyn_agree_ren_refl Γ Δ :
-  dyn_wf Γ Δ -> dyn_agree_ren id Γ Δ Γ Δ.
-Proof with eauto using dyn_agree_ren.
+Lemma program_agree_ren_refl Γ Δ :
+  program_wf Γ Δ -> program_agree_ren id Γ Δ Γ Δ.
+Proof with eauto using program_agree_ren.
   elim: Γ Δ.
   { move=>Δ wf. inv wf... }
   { move=>A Γ ih Δ wf. inv wf.
     { have agr:=ih _ H1.
-      have:dyn_agree_ren (upren id)
+      have:program_agree_ren (upren id)
         (A :: Γ) (A :{s} Δ0) (A.[ren id] :: Γ) (A.[ren id] :{s} Δ0)...
       by asimpl. }
     { have agr:=ih _ H1.
-      have:dyn_agree_ren (upren id)
+      have:program_agree_ren (upren id)
         (A :: Γ) (_: Δ0) (A.[ren id] :: Γ) (_: Δ0)...
       by asimpl. } }
 Qed.
 
-Lemma dyn_agree_ren_key Γ Γ' Δ Δ' ξ s :
-  dyn_agree_ren ξ Γ Δ Γ' Δ' -> Δ ▷ s -> Δ' ▷ s.
+Lemma program_agree_ren_key Γ Γ' Δ Δ' ξ s :
+  program_agree_ren ξ Γ Δ Γ' Δ' -> Δ ▷ s -> Δ' ▷ s.
 Proof with eauto using key.
   move=>agr. elim: agr s=>{Γ Γ' Δ Δ' ξ}...
   { move=>Γ Γ' Δ Δ' ξ m s tym agr ih t k. inv k... }
@@ -60,9 +63,9 @@ Proof with eauto using key.
   { move=>Γ Γ' Δ Δ' ξ m _ agr ih [] /ih... }
 Qed.
 
-Lemma dyn_agree_ren_has Γ Γ' Δ Δ' ξ x s A :
-  dyn_agree_ren ξ Γ Δ Γ' Δ' -> dyn_has Δ x s A -> dyn_has Δ' (ξ x) s A.[ren ξ].
-Proof with eauto using dyn_agree_ren_key.
+Lemma program_agree_ren_has Γ Γ' Δ Δ' ξ x s A :
+  program_agree_ren ξ Γ Δ Γ' Δ' -> program_has Δ x s A -> program_has Δ' (ξ x) s A.[ren ξ].
+Proof with eauto using program_agree_ren_key.
   move=>agr. elim: agr x s A=>{Γ Γ' Δ Δ' ξ}.
   { move=>ξ x s A hs. inv hs. }
   { move=>Γ Γ' Δ Δ' ξ m s tym agr ih x t A hs. inv hs; asimpl.
@@ -81,13 +84,13 @@ Proof with eauto using dyn_agree_ren_key.
     constructor... }
 Qed.
 
-Lemma dyn_agree_ren_merge Γ Γ' Δ Δ' Δ1 Δ2 ξ :
-  dyn_agree_ren ξ Γ Δ Γ' Δ' -> Δ1 ∘ Δ2 => Δ ->
+Lemma program_agree_ren_merge Γ Γ' Δ Δ' Δ1 Δ2 ξ :
+  program_agree_ren ξ Γ Δ Γ' Δ' -> Δ1 ∘ Δ2 => Δ ->
   ∃ Δ1' Δ2',
     Δ1' ∘ Δ2' => Δ' /\
-    dyn_agree_ren ξ Γ Δ1 Γ' Δ1' /\
-    dyn_agree_ren ξ Γ Δ2 Γ' Δ2'.
-Proof with eauto 6 using merge, dyn_agree_ren.
+    program_agree_ren ξ Γ Δ1 Γ' Δ1' /\
+    program_agree_ren ξ Γ Δ2 Γ' Δ2'.
+Proof with eauto 6 using merge, program_agree_ren.
   move=>agr. elim: agr Δ1 Δ2=>{Γ Γ' Δ Δ' ξ}.
   { move=>ξ Δ1 Δ2 mrg. inv mrg.
     exists nil. exists nil... }
@@ -112,196 +115,201 @@ Proof with eauto 6 using merge, dyn_agree_ren.
     exists (_: Δ1'). exists (_: Δ2')... }
 Qed.
 
-Lemma dyn_agree_weak_wf_nil Γ' Δ' ξ :
-  dyn_agree_ren ξ nil nil Γ' Δ' -> dyn_wf Γ' Δ'.
-Proof with eauto using dyn_wf.
+Lemma program_agree_weak_wf_nil Γ' Δ' ξ :
+  program_agree_ren ξ nil nil Γ' Δ' -> program_wf Γ' Δ'.
+Proof with eauto using program_wf.
   move e1:(nil)=>Γ.
   move e2:(nil)=>Δ agr.
   elim: agr e1 e2=>//{Γ Γ' Δ Δ' ξ}...
 Qed.
 
-Lemma dyn_agree_weak_wf_ty Γ Γ' Δ Δ' A s ξ :
-  dyn_agree_ren ξ (A :: Γ) (A :{s} Δ) Γ' Δ' -> dyn_wf Γ Δ ->
-  (∀ Γ' Δ' ξ, dyn_agree_ren ξ Γ Δ Γ' Δ' → dyn_wf Γ' Δ') ->
-  dyn_wf Γ' Δ'.
-Proof with eauto using dyn_wf.
+Lemma program_agree_weak_wf_ty Γ Γ' Δ Δ' A s ξ :
+  program_agree_ren ξ (A :: Γ) (A :{s} Δ) Γ' Δ' -> program_wf Γ Δ ->
+  (∀ Γ' Δ' ξ, program_agree_ren ξ Γ Δ Γ' Δ' → program_wf Γ' Δ') ->
+  program_wf Γ' Δ'.
+Proof with eauto using program_wf.
   move e1:(A :: Γ)=>Γ0.
   move e2:(A :{s} Δ)=>Δ0 agr.
   elim: agr A Γ Δ s e1 e2=>//{Γ0 Δ0 Γ' Δ' ξ}...
   move=>Γ Γ' Δ Δ' ξ m s tym agr _ A Γ0 Δ0 s0[e1 e2][_ e4 e5]wf h; subst.
-  apply: dyn_wf_ty...
+  apply: program_wf_ty...
   replace (Sort s) with (Sort s).[ren ξ] by eauto.
-  apply: sta_rename...
-  apply: dyn_sta_agree_ren...
+  apply: logical_rename...
+  apply: program_logical_agree_ren...
 Qed.
 
-Lemma dyn_agree_weak_wf_n Γ Γ' Δ Δ' A ξ :
-  dyn_agree_ren ξ (A :: Γ) (_: Δ) Γ' Δ' -> dyn_wf Γ Δ ->
-  (∀ Γ' Δ' ξ, dyn_agree_ren ξ Γ Δ Γ' Δ' → dyn_wf Γ' Δ') ->
-  dyn_wf Γ' Δ'.
-Proof with eauto using dyn_wf.
+Lemma program_agree_weak_wf_n Γ Γ' Δ Δ' A ξ :
+  program_agree_ren ξ (A :: Γ) (_: Δ) Γ' Δ' -> program_wf Γ Δ ->
+  (∀ Γ' Δ' ξ, program_agree_ren ξ Γ Δ Γ' Δ' → program_wf Γ' Δ') ->
+  program_wf Γ' Δ'.
+Proof with eauto using program_wf.
   move e1:(A :: Γ)=>Γ0.
   move e2:(_: Δ)=>Δ0 agr.
   elim: agr A Γ Δ e1 e2=>//{Γ0 Δ0 Γ' Δ' ξ}...
   move=>Γ Γ' Δ Δ' ξ m s tym agr _ A Γ0 Δ0 [e1 e2][e4]wf h; subst.
-  apply: dyn_wf_n...
-  have:=sta_rename tym (dyn_sta_agree_ren agr).
+  apply: program_wf_n...
+  have:=logical_rename tym (program_logical_agree_ren agr).
   asimpl...
 Qed.
 
-Lemma dyn_rename Γ Γ' Δ Δ' m A ξ :
-  Γ ; Δ ⊢ m : A -> dyn_agree_ren ξ Γ Δ Γ' Δ' -> Γ' ; Δ' ⊢ m.[ren ξ] : A.[ren ξ].
+(* Generalized renaming lemma. *)
+Lemma program_rename Γ Γ' Δ Δ' m A ξ :
+  Γ ; Δ ⊢ m : A -> program_agree_ren ξ Γ Δ Γ' Δ' -> Γ' ; Δ' ⊢ m.[ren ξ] : A.[ren ξ].
 Proof with eauto using
-  dyn_type, sta_agree_ren, dyn_agree_ren, dyn_agree_ren_key.
+  program_type, logical_agree_ren, program_agree_ren, program_agree_ren_key.
   move=>ty. move: Γ Δ m A ty Γ' Δ' ξ.
-  apply:(@dyn_type_mut _
-    (fun Γ Δ wf => forall Γ' Δ' ξ, dyn_agree_ren ξ Γ Δ Γ' Δ' -> dyn_wf Γ' Δ')).
+  apply:(@program_type_mut _
+    (fun Γ Δ wf => forall Γ' Δ' ξ, program_agree_ren ξ Γ Δ Γ' Δ' -> program_wf Γ' Δ')).
   { move=>Γ Δ x s A wf h shs dhs Γ' Δ' ξ agr. asimpl.
-    apply: dyn_var...
-    apply: sta_agree_ren_has...
-    apply: dyn_sta_agree_ren...
-    apply: dyn_agree_ren_has... }
+    apply: program_var...
+    apply: logical_agree_ren_has...
+    apply: program_logical_agree_ren...
+    apply: program_agree_ren_has... }
   { move=>Γ Δ A B m s k tym ihm Γ' Δ' ξ agr. asimpl.
-    have wf:=dyn_type_wf tym. inv wf.
-    apply: dyn_lam0... }
+    have wf:=program_type_wf tym. inv wf.
+    apply: program_lam0... }
   { move=>Γ Δ A B m s t k tym ihm Γ' Δ' ξ agr. asimpl.
-    have wf:=dyn_type_wf tym. inv wf.
-    apply: dyn_lam1... }
+    have wf:=program_type_wf tym. inv wf.
+    apply: program_lam1... }
   { move=>Γ Δ A B m n s tym ihm tyn Γ' Δ' ξ agr. asimpl.
     replace B.[n.[ren ξ] .: ren ξ] with B.[ren (upren ξ)].[n.[ren ξ]/]
       by autosubst.
     have{}ihm:=ihm _ _ _ agr.
-    have{}ihn:=sta_rename tyn (dyn_sta_agree_ren agr).
-    apply: dyn_app0...
+    have{}ihn:=logical_rename tyn (program_logical_agree_ren agr).
+    apply: program_app0...
     asimpl in ihm... }
   { move=>Γ Δ1 Δ2 Δ A B m n s mrg tym ihm tyn ihn Γ' Δ' ξ agr. asimpl.
     replace B.[n.[ren ξ] .: ren ξ] with B.[ren (upren ξ)].[n.[ren ξ]/]
       by autosubst.
-    have[Δ1'[Δ2'[mrg'[agr1 agr2]]]]:=dyn_agree_ren_merge agr mrg.
+    have[Δ1'[Δ2'[mrg'[agr1 agr2]]]]:=program_agree_ren_merge agr mrg.
     have{}ihm:=ihm _ _ _ agr1.
     have{}ihn:=ihn _ _ _ agr2.
-    apply: dyn_app1...
+    apply: program_app1...
     asimpl in ihm... }
   { move=>Γ Δ A B m n t tyS tym ihm tyn Γ' Δ' ξ agr. asimpl.
     have{}ihm:=ihm _ _ _ agr.
-    have{}ihn:=sta_rename tyn (dyn_sta_agree_ren agr).
-    have{}ihS:=sta_rename tyS (dyn_sta_agree_ren agr).
-    apply: dyn_pair0...
+    have{}ihn:=logical_rename tyn (program_logical_agree_ren agr).
+    have{}ihS:=logical_rename tyS (program_logical_agree_ren agr).
+    apply: program_pair0...
     asimpl in ihS...
     asimpl. asimpl in ihn... }
   { move=>Γ Δ1 Δ2 Δ A B m n t mrg tyS tym ihm tyn ihn Γ' Δ' ξ agr. asimpl.
-    have[Δ1'[Δ2'[mrg'[agr1 agr2]]]]:=dyn_agree_ren_merge agr mrg.
+    have[Δ1'[Δ2'[mrg'[agr1 agr2]]]]:=program_agree_ren_merge agr mrg.
     have{}ihm:=ihm _ _ _ agr1.
     have{}ihn:=ihn _ _ _ agr2.
-    have{}ihS:=sta_rename tyS (dyn_sta_agree_ren agr).
-    apply: dyn_pair1...
+    have{}ihS:=logical_rename tyS (program_logical_agree_ren agr).
+    apply: program_pair1...
     asimpl in ihS...
     asimpl. asimpl in ihn... }
   { move=>Γ Δ1 Δ2 Δ A B C m n s r t mrg tyC tym ihm tyn ihn Γ' Δ' ξ agr. asimpl.
-    have wf:=sta_type_wf tyC. inv wf.
-    have wf:=dyn_type_wf tyn. inv wf. inv H4.
-    have[Δ1'[Δ2'[mrg'[agr1 agr2]]]]:=dyn_agree_ren_merge agr mrg.
-    have{}ihC:=sta_rename tyC (sta_agree_ren_cons H2 (dyn_sta_agree_ren agr)).
+    have wf:=logical_type_wf tyC. inv wf.
+    have wf:=program_type_wf tyn. inv wf. inv H4.
+    have[Δ1'[Δ2'[mrg'[agr1 agr2]]]]:=program_agree_ren_merge agr mrg.
+    have{}ihC:=logical_rename tyC (logical_agree_ren_cons H2 (program_logical_agree_ren agr)).
     have{}ihm:=ihm _ _ _ agr1.
-    have/ihn{}ihn:dyn_agree_ren (upren (upren ξ)) (B :: A :: Γ) (_: A :{r} Δ2)
+    have/ihn{}ihn:program_agree_ren (upren (upren ξ)) (B :: A :: Γ) (_: A :{r} Δ2)
       (B.[ren (upren ξ)] :: A.[ren ξ] :: Γ') (_: A.[ren ξ] :{r} Δ2')...
     asimpl in ihC.
     asimpl in ihm.
     replace C.[Pair0 (Var 1) (Var 0) t .: ren (+2)].[ren (upren (upren ξ))]
       with C.[ren (upren ξ)].[Pair0 (Var 1) (Var 0) t .: ren (+2)]
         in ihn by autosubst.
-    have:=dyn_letin0 mrg' ihC ihm ihn.
+    have:=program_letin0 mrg' ihC ihm ihn.
     by autosubst. }
   { move=>Γ Δ1 Δ2 Δ A B C m n s r1 r2 t mrg tyC tym ihm tyn ihn Γ' Δ' ξ agr. asimpl.
-    have wf:=sta_type_wf tyC. inv wf.
-    have wf:=dyn_type_wf tyn. inv wf. inv H4.
-    have[Δ1'[Δ2'[mrg'[agr1 agr2]]]]:=dyn_agree_ren_merge agr mrg.
-    have{}ihC:=sta_rename tyC (sta_agree_ren_cons H2 (dyn_sta_agree_ren agr)).
+    have wf:=logical_type_wf tyC. inv wf.
+    have wf:=program_type_wf tyn. inv wf. inv H4.
+    have[Δ1'[Δ2'[mrg'[agr1 agr2]]]]:=program_agree_ren_merge agr mrg.
+    have{}ihC:=logical_rename tyC (logical_agree_ren_cons H2 (program_logical_agree_ren agr)).
     have{}ihm:=ihm _ _ _ agr1.
-    have/ihn{}ihn:dyn_agree_ren (upren (upren ξ)) (B :: A :: Γ) (B :{r2} A :{r1} Δ2)
+    have/ihn{}ihn:program_agree_ren (upren (upren ξ)) (B :: A :: Γ) (B :{r2} A :{r1} Δ2)
       (B.[ren (upren ξ)] :: A.[ren ξ] :: Γ') (B.[ren (upren ξ)] :{r2} A.[ren ξ] :{r1} Δ2')...
     asimpl in ihC.
     asimpl in ihm.
     replace C.[Pair1 (Var 1) (Var 0) t .: ren (+2)].[ren (upren (upren ξ))]
       with C.[ren (upren ξ)].[Pair1 (Var 1) (Var 0) t .: ren (+2)]
         in ihn by autosubst.
-    have:=dyn_letin1 mrg' ihC ihm ihn.
+    have:=program_letin1 mrg' ihC ihm ihn.
     by autosubst. }
-  { move=>Γ Δ A B m n t k tym ihm tyn ihn Γ' Δ' ξ agr. asimpl. apply:dyn_apair... }
-  { move=>Γ Δ A B m t tym ihm Γ' Δ' ξ agr. asimpl. apply:dyn_fst... }
-  { move=>Γ Δ A B m t tym ihm Γ' Δ' ξ agr. asimpl. apply:dyn_snd... }
+  { move=>Γ Δ A B m n t k tym ihm tyn ihn Γ' Δ' ξ agr. asimpl. apply:program_apair... }
+  { move=>Γ Δ A B m t tym ihm Γ' Δ' ξ agr. asimpl. apply:program_fst... }
+  { move=>Γ Δ A B m t tym ihm Γ' Δ' ξ agr. asimpl. apply:program_snd... }
   { move=>Γ Δ A B H P m n s tyB tyH ihH tyP Γ' Δ' ξ agr. asimpl.
-    have wf:=sta_type_wf tyB. inv wf. inv H2.
-    have ihP:=sta_rename tyP (dyn_sta_agree_ren agr).
-    have agr':=dyn_sta_agree_ren agr.
+    have wf:=logical_type_wf tyB. inv wf. inv H2.
+    have ihP:=logical_rename tyP (program_logical_agree_ren agr).
+    have agr':=program_logical_agree_ren agr.
     have{}agr':
-      sta_agree_ren (upren (upren ξ))
+      logical_agree_ren (upren (upren ξ))
         (Id A.[ren (+1)] m.[ren (+1)] (Var 0) :: A :: Γ)
         ((Id A.[ren (+1)] m.[ren (+1)] (Var 0)).[ren (upren ξ)] :: A.[ren ξ] :: Γ')...
-    have ihB:=sta_rename tyB agr'.
+    have ihB:=logical_rename tyB agr'.
     have{}ihH:=ihH _ _ _ agr.
     asimpl in ihP.
     asimpl in ihB.
     asimpl in ihH.
     replace A.[ren (ξ >>> (+1))] with A.[ren ξ].[ren (+1)] in ihB by autosubst.
     replace m.[ren (ξ >>> (+1))] with m.[ren ξ].[ren (+1)] in ihB by autosubst.
-    have pf:=dyn_rw ihB. asimpl in pf.
+    have pf:=program_rw ihB. asimpl in pf.
     have:=pf _ _ _ _ ihH ihP.
     by autosubst. }
   { move=>Γ Δ A B m s eq tym ihm tyB Γ' Δ' ξ agr.
-    apply: dyn_conv.
-    apply: sta_conv_subst...
+    apply: program_conv.
+    apply: logical_conv_subst...
     apply: ihm...
-    have:=sta_rename tyB (dyn_sta_agree_ren agr).
+    have:=logical_rename tyB (program_logical_agree_ren agr).
     asimpl... }
-  { exact: dyn_agree_weak_wf_nil... }
+  { exact: program_agree_weak_wf_nil... }
   { move=>Γ Δ A s wf ih tyA Γ' Δ' ξ agr.
-    apply: dyn_agree_weak_wf_ty... }
+    apply: program_agree_weak_wf_ty... }
   { move=>Γ Δ A s wf ih tyA Γ' Δ' ξ agr.
-    apply: dyn_agree_weak_wf_n... }
+    apply: program_agree_weak_wf_n... }
 Qed.
 
-Lemma dyn_rename_wf Γ Γ' Δ Δ' ξ :
-  dyn_wf Γ Δ -> dyn_agree_ren ξ Γ Δ Γ' Δ' -> dyn_wf Γ' Δ'.
-Proof with eauto using dyn_wf.
+Lemma program_rename_wf Γ Γ' Δ Δ' ξ :
+  program_wf Γ Δ -> program_agree_ren ξ Γ Δ Γ' Δ' -> program_wf Γ' Δ'.
+Proof with eauto using program_wf.
   move=>wf. elim: wf Γ' Δ' ξ=>{Γ Δ}.
-  { move=>*. apply: dyn_agree_weak_wf_nil... }
-  { move=>*. apply: dyn_agree_weak_wf_ty... }
-  { move=>*. apply: dyn_agree_weak_wf_n... }
+  { move=>*. apply: program_agree_weak_wf_nil... }
+  { move=>*. apply: program_agree_weak_wf_ty... }
+  { move=>*. apply: program_agree_weak_wf_n... }
 Qed.
 
-Lemma dyn_weakenU Γ Δ m A B :
-  Γ ⊢ B : Sort U ->
-  Γ ; Δ ⊢ m : A ->
-  (B :: Γ) ; B :U Δ ⊢ m.[ren (+1)] : A.[ren (+1)].
-Proof with eauto using dyn_agree_ren, dyn_agree_ren_refl.
-  move=>tyB tym. apply: dyn_rename...
-Qed.
-
-Lemma dyn_weakenN Γ Δ m A B s :
+(* Lemma 3 (Program 0-Weakening) *)
+Lemma program_weaken0 Γ Δ m A B s :
   Γ ⊢ B : Sort s ->
   Γ ; Δ ⊢ m : A ->
   (B :: Γ) ; _: Δ ⊢ m.[ren (+1)] : A.[ren (+1)].
-Proof with eauto using dyn_agree_ren, dyn_agree_ren_refl.
-  move=>tyB tym. apply: dyn_rename...
+Proof with eauto using program_agree_ren, program_agree_ren_refl.
+  move=>tyB tym. apply: program_rename...
 Qed.
 
-Lemma dyn_eweakenU Γ Δ m m' A A' B :
-  m' = m.[ren (+1)] ->
-  A' = A.[ren (+1)] ->
+(* Lemma 4 (Program 1-Weakening) *)
+Lemma program_weaken1 Γ Δ m A B :
   Γ ⊢ B : Sort U ->
   Γ ; Δ ⊢ m : A ->
-  (B :: Γ) ; B :U Δ ⊢ m' : A'.
-Proof.
-  move=>*; subst. exact: dyn_weakenU.
+  (B :: Γ) ; B :U Δ ⊢ m.[ren (+1)] : A.[ren (+1)].
+Proof with eauto using program_agree_ren, program_agree_ren_refl.
+  move=>tyB tym. apply: program_rename...
 Qed.
 
-Lemma dyn_eweakenN Γ Δ m m' A A' B s :
+(* Alternative statement more suitable for certain Coq tactics *)
+Lemma program_eweaken0 Γ Δ m m' A A' B s :
   m' = m.[ren (+1)] ->
   A' = A.[ren (+1)] ->
   Γ ⊢ B : Sort s ->
   Γ ; Δ ⊢ m : A ->
   (B :: Γ) ; _: Δ ⊢ m' : A'.
 Proof.
-  move=>*; subst. apply: dyn_weakenN; eauto.
+  move=>*; subst. apply: program_weaken0; eauto.
+Qed.
+
+(* Alternative statement more suitable for certain Coq tactics *)
+Lemma program_eweaken1 Γ Δ m m' A A' B :
+  m' = m.[ren (+1)] ->
+  A' = A.[ren (+1)] ->
+  Γ ⊢ B : Sort U ->
+  Γ ; Δ ⊢ m : A ->
+  (B :: Γ) ; B :U Δ ⊢ m' : A'.
+Proof.
+  move=>*; subst. exact: program_weaken1.
 Qed.
