coq/theories/logical_inv.v
@@ -1,12 +1,14 @@
+(* The file presents various inversion lemmas for the logical level. *)
+
 From mathcomp Require Import ssreflect ssrbool eqtype ssrnat seq.
 From Coq Require Import ssrfun Classical Utf8.
-Require Export AutosubstSsr ARS sta_subst.
+Require Export AutosubstSsr ARS logical_subst.
 
 Set Implicit Arguments.
 Unset Strict Implicit.
 Unset Printing Implicit Defensive.
 
-Lemma sta_pi0_inv Γ A B C s :
+Lemma logical_pi0_inv Γ A B C s :
   Γ ⊢ Pi0 A B s : C ->
   exists t, (A :: Γ) ⊢ B : Sort t /\ C === Sort s.
 Proof with eauto.
@@ -22,7 +24,7 @@ Proof with eauto.
     exact: eq2. }
 Qed.
 
-Lemma sta_pi1_inv Γ A B C s :
+Lemma logical_pi1_inv Γ A B C s :
   Γ ⊢ Pi1 A B s : C ->
   exists t, (A :: Γ) ⊢ B : Sort t /\ C === Sort s.
 Proof with eauto.
@@ -38,7 +40,7 @@ Proof with eauto.
     exact: eq2. }
 Qed.
 
-Lemma sta_sig0_inv Γ A B C t :
+Lemma logical_sig0_inv Γ A B C t :
   Γ ⊢ Sig0 A B t : C ->
   exists s r, s ⊑ t /\ Γ ⊢ A : Sort s /\ (A :: Γ) ⊢ B : Sort r /\ C === Sort t.
 Proof with eauto.
@@ -54,7 +56,7 @@ Proof with eauto.
     exact: eq'. }
 Qed.
 
-Lemma sta_sig1_inv Γ A B C t :
+Lemma logical_sig1_inv Γ A B C t :
   Γ ⊢ Sig1 A B t : C ->
   exists s r,
     s ⊑ t /\ r ⊑ t /\
@@ -72,7 +74,7 @@ Proof with eauto.
     exact: eq'. }
 Qed.
 
-Lemma sta_with_inv Γ A B C t :
+Lemma logical_with_inv Γ A B C t :
   Γ ⊢ With A B t : C ->
   exists s r, Γ ⊢ A : Sort s /\ Γ ⊢ B : Sort r /\ C === Sort t.
 Proof with eauto.
@@ -88,7 +90,7 @@ Proof with eauto.
     exact: eq'. }
 Qed.
 
-Lemma sta_id_inv Γ A B m n :
+Lemma logical_id_inv Γ A B m n :
   Γ ⊢ Id A m n : B ->
   Γ ⊢ m : A /\ Γ ⊢ n : A /\ B === Sort U.
 Proof with eauto.
@@ -103,7 +105,7 @@ Proof with eauto.
     exact: eq'. }
 Qed.
 
-Lemma sta_lam0_pi1_false Γ A1 A2 B C m s1 s2 :
+Lemma logical_lam0_pi1_false Γ A1 A2 B C m s1 s2 :
   Γ ⊢ Lam0 A1 m s1 : C -> C === Pi1 A2 B s2 -> False.
 Proof with eauto.
   move e:(Lam0 A1 m s1)=>n tyL.
@@ -114,7 +116,7 @@ Proof with eauto.
     apply: conv_trans... }
 Qed.
 
-Lemma sta_lam1_pi0_false Γ A1 A2 B C m s1 s2 :
+Lemma logical_lam1_pi0_false Γ A1 A2 B C m s1 s2 :
   Γ ⊢ Lam1 A1 m s1 : C -> C === Pi0 A2 B s2 -> False.
 Proof with eauto.
   move e:(Lam1 A1 m s1)=>n tyL.
@@ -125,7 +127,7 @@ Proof with eauto.
     apply: conv_trans... }
 Qed.
 
-Lemma sta_pair0_sig1_false Γ A B C m1 m2 s1 s2 :
+Lemma logical_pair0_sig1_false Γ A B C m1 m2 s1 s2 :
   Γ ⊢ Pair0 m1 m2 s1 : C -> C === Sig1 A B s2 -> False.
 Proof with eauto.
   move e:(Pair0 m1 m2 s1)=>n tyP.
@@ -136,7 +138,7 @@ Proof with eauto.
     apply: conv_trans... }
 Qed.
 
-Lemma sta_pair1_sig0_false Γ A B C m1 m2 s1 s2 :
+Lemma logical_pair1_sig0_false Γ A B C m1 m2 s1 s2 :
   Γ ⊢ Pair1 m1 m2 s1 : C -> C === Sig0 A B s2 -> False.
 Proof with eauto.
   move e:(Pair1 m1 m2 s1)=>n tyP.
