coq/theories/logical_sr.v
@@ -1,391 +1,395 @@
+(* This file presents the subject reduction theorem of the logical level. *)
+
 From mathcomp Require Import ssreflect ssrbool eqtype ssrnat seq.
 From Coq Require Import ssrfun Classical Utf8.
-Require Export AutosubstSsr ARS sta_valid.
+Require Export AutosubstSsr ARS logical_valid.
 
 Set Implicit Arguments.
 Unset Strict Implicit.
 Unset Printing Implicit Defensive.
 
-Theorem sta_sr Γ m n A : Γ ⊢ m : A -> m ~> n -> Γ ⊢ n : A.
-Proof with eauto using sta0_type, sta0_wf, sta_step, sta_type.
-  move=>/sta_sta0_type ty st. apply: sta0_sta_type.
+(* Theorem 4 (Logical Subject Reduction) *)
+Theorem logical_sr Γ m n A : Γ ⊢ m : A -> m ~> n -> Γ ⊢ n : A.
+Proof with eauto using logical0_type, logical0_wf, logical_step, logical_type.
+  move=>/logical_logical0_type ty st. apply: logical0_logical_type.
   elim: ty n st=>{Γ m A}...
   { move=>Γ s wf n st. inv st. }
   { move=>Γ x A wf hs n st. inv st. }
   { move=>Γ A B s r t tyA ihA tyB ihB n st. inv st.
     { have tyA':=ihA _ H3.
-      apply: sta0_pi0...
-      apply: sta_sta0_type.
-      move/sta0_sta_type in tyB.
-      move/sta0_sta_type in tyA'.
-      apply: sta_ctx_conv.
+      apply: logical0_pi0...
+      apply: logical_logical0_type.
+      move/logical0_logical_type in tyB.
+      move/logical0_logical_type in tyA'.
+      apply: logical_ctx_conv.
       apply: conv1i...
       exact: tyA'.
       exact: tyB. }
     { have tyB':=ihB _ H3.
-      apply: sta0_pi0... } }
+      apply: logical0_pi0... } }
   { move=>Γ A B s r t tyA ihA tyB ihB n st. inv st.
     { have tyA':=ihA _ H3.
-      apply: sta0_pi1...
-      apply: sta_sta0_type.
-      move/sta0_sta_type in tyB.
-      move/sta0_sta_type in tyA'.
-      apply: sta_ctx_conv.
+      apply: logical0_pi1...
+      apply: logical_logical0_type.
+      move/logical0_logical_type in tyB.
+      move/logical0_logical_type in tyA'.
+      apply: logical_ctx_conv.
       apply: conv1i...
       exact: tyA'.
       exact: tyB. }
     { have tyB':=ihB _ H3.
-      apply: sta0_pi1... } }
+      apply: logical0_pi1... } }
   { move=>Γ A B m s r tyA ihA tym ihm n st. inv st.
     { have tyA':=ihA _ H3.
-      move/sta0_sta_type in tym.
-      move/sta0_sta_type in tyA'.
-      have[t tyB]:=sta_valid tym.
-      apply: sta0_conv.
+      move/logical0_logical_type in tym.
+      move/logical0_logical_type in tyA'.
+      have[t tyB]:=logical_valid tym.
+      apply: logical0_conv.
       apply: conv1i...
-      apply: sta0_lam0...
-      apply: sta_sta0_type.
-      apply: sta_ctx_conv.
+      apply: logical0_lam0...
+      apply: logical_logical0_type.
+      apply: logical_ctx_conv.
       apply: conv1i...
       exact: tyA'.
       exact: tym.
-      apply: sta0_pi0... }
+      apply: logical0_pi0... }
     { have tym':=ihm _ H3.
-      apply: sta0_lam0... } }
+      apply: logical0_lam0... } }
   { move=>Γ A B m s r tyA ihA tym ihm n st. inv st.
     { have tyA':=ihA _ H3.
-      move/sta0_sta_type in tym.
-      move/sta0_sta_type in tyA'.
-      have[t tyB]:=sta_valid tym.
-      apply: sta0_conv.
+      move/logical0_logical_type in tym.
+      move/logical0_logical_type in tyA'.
+      have[t tyB]:=logical_valid tym.
+      apply: logical0_conv.
       apply: conv1i...
-      apply: sta0_lam1...
-      apply: sta_sta0_type.
-      apply: sta_ctx_conv.
+      apply: logical0_lam1...
+      apply: logical_logical0_type.
+      apply: logical_ctx_conv.
       apply: conv1i...
       exact: tyA'.
       exact: tym.
-      apply: sta0_pi1... }
+      apply: logical0_pi1... }
     { have tym':=ihm _ H3.
-      apply: sta0_lam1... } }
+      apply: logical0_lam1... } }
   { move=>Γ A B m n s tym ihm tyn ihn x st. inv st.
     { have tym':=ihm _ H2... }
     { have tyn':=ihn _ H2.
-      move/sta0_sta_type in tyn.
-      have[_/sta_pi0_inv[r[tyB _]]]:=sta_valid (sta0_sta_type tym).
-      apply: sta0_conv.
-      apply: sta_conv_beta.
+      move/logical0_logical_type in tyn.
+      have[_/logical_pi0_inv[r[tyB _]]]:=logical_valid (logical0_logical_type tym).
+      apply: logical0_conv.
+      apply: logical_conv_beta.
       apply: conv1i...
-      apply: sta0_app0...
-      apply: sta_sta0_type.
-      apply: sta_esubst...
+      apply: logical0_app0...
+      apply: logical_logical0_type.
+      apply: logical_esubst...
       by autosubst. }
-    { have[x tyP]:=sta_valid (sta0_sta_type tym).
-      have/sta_lam0_inv tym0:=sta0_sta_type tym.
-      move/sta0_sta_type in tyn.
-      apply: sta_sta0_type.
-      apply: sta_esubst... }
-    { exfalso. apply: sta_lam1_pi0_false.
-      apply: sta0_sta_type... eauto. } }
+    { have[x tyP]:=logical_valid (logical0_logical_type tym).
+      have/logical_lam0_inv tym0:=logical0_logical_type tym.
+      move/logical0_logical_type in tyn.
+      apply: logical_logical0_type.
+      apply: logical_esubst... }
+    { exfalso. apply: logical_lam1_pi0_false.
+      apply: logical0_logical_type... eauto. } }
   { move=>Γ A B m n s tym ihm tyn ihn x st. inv st.
     { have tym':=ihm _ H2... }
     { have tyn':=ihn _ H2.
-      move/sta0_sta_type in tyn.
-      have[_/sta_pi1_inv[r[tyB _]]]:=sta_valid (sta0_sta_type tym).
-      apply: sta0_conv.
-      apply: sta_conv_beta.
+      move/logical0_logical_type in tyn.
+      have[_/logical_pi1_inv[r[tyB _]]]:=logical_valid (logical0_logical_type tym).
+      apply: logical0_conv.
+      apply: logical_conv_beta.
       apply: conv1i...
-      apply: sta0_app1...
-      apply: sta_sta0_type.
-      apply: sta_esubst...
+      apply: logical0_app1...
+      apply: logical_logical0_type.
+      apply: logical_esubst...
       by autosubst. }
-    { exfalso. apply: sta_lam0_pi1_false.
-      apply: sta0_sta_type... eauto. } 
-    { have[x tyP]:=sta_valid (sta0_sta_type tym).
-      have/sta_lam1_inv tym0:=sta0_sta_type tym.
-      move/sta0_sta_type in tyn.
-      apply: sta_sta0_type.
-      apply: sta_esubst... } }
+    { exfalso. apply: logical_lam0_pi1_false.
+      apply: logical0_logical_type... eauto. } 
+    { have[x tyP]:=logical_valid (logical0_logical_type tym).
+      have/logical_lam1_inv tym0:=logical0_logical_type tym.
+      move/logical0_logical_type in tyn.
+      apply: logical_logical0_type.
+      apply: logical_esubst... } }
   { move=>Γ A B s r t ord tyA ihA tyB ihB n st. inv st.
     { have tyA':=ihA _ H3.
-      move/sta0_sta_type in tyB.
-      move/sta0_sta_type in tyA'.
-      apply: sta0_sig0...
-      apply: sta_sta0_type.
-      apply: sta_ctx_conv.
+      move/logical0_logical_type in tyB.
+      move/logical0_logical_type in tyA'.
+      apply: logical0_sig0...
+      apply: logical_logical0_type.
+      apply: logical_ctx_conv.
       apply: conv1i...
       apply: tyA'.
       apply: tyB. }
     { have tyB':=ihB _ H3.
-      apply: sta0_sig0... } }
+      apply: logical0_sig0... } }
   { move=>Γ A B s r t ord1 ord2 tyA ihA tyB ihB n st. inv st.
     { have tyA':=ihA _ H3.
-      move/sta0_sta_type in tyB.
-      move/sta0_sta_type in tyA'.
-      apply: sta0_sig1.
+      move/logical0_logical_type in tyB.
+      move/logical0_logical_type in tyA'.
+      apply: logical0_sig1.
       apply: ord1. apply: ord2.
       eauto.
-      apply: sta_sta0_type.
-      apply: sta_ctx_conv.
+      apply: logical_logical0_type.
+      apply: logical_ctx_conv.
       apply: conv1i...
       apply: tyA'.
       apply: tyB. }
     { have tyB':=ihB _ H3.
-      apply: sta0_sig1.
+      apply: logical0_sig1.
       apply: ord1. apply: ord2.
       all: eauto. } }
   { move=>Γ A B m n t tyS ihS tym ihm tyn ihn x st. inv st.
-    { have/sta0_sta_type tym':=ihm _ H3.
-      have tyS':=sta0_sta_type tyS.
-      have[s[r[ord[tyA[tyB _]]]]]:=sta_sig0_inv tyS'.
-      apply: sta0_pair0...
-      apply: sta0_conv.
-      apply: sta_conv_beta.
+    { have/logical0_logical_type tym':=ihm _ H3.
+      have tyS':=logical0_logical_type tyS.
+      have[s[r[ord[tyA[tyB _]]]]]:=logical_sig0_inv tyS'.
+      apply: logical0_pair0...
+      apply: logical0_conv.
+      apply: logical_conv_beta.
       apply: conv1...
       apply: tyn.
-      apply: sta_sta0_type.
-      apply: sta_esubst...
+      apply: logical_logical0_type.
+      apply: logical_esubst...
       by autosubst. }
     { have tyn':=ihn _ H3.
-      apply: sta0_pair0... } }
+      apply: logical0_pair0... } }
   { move=>Γ A B m n t tyS ihS tym ihm tyn ihn x st. inv st.
-    { have/sta0_sta_type tym':=ihm _ H3.
-      have tyS':=sta0_sta_type tyS.
-      have[s[r[ord1[ord2[tyA[tyB _]]]]]]:=sta_sig1_inv tyS'.
-      apply: sta0_pair1...
-      apply: sta0_conv.
-      apply: sta_conv_beta.
+    { have/logical0_logical_type tym':=ihm _ H3.
+      have tyS':=logical0_logical_type tyS.
+      have[s[r[ord1[ord2[tyA[tyB _]]]]]]:=logical_sig1_inv tyS'.
+      apply: logical0_pair1...
+      apply: logical0_conv.
+      apply: logical_conv_beta.
       apply: conv1...
       apply: tyn.
-      apply: sta_sta0_type.
-      apply: sta_esubst...
+      apply: logical_logical0_type.
+      apply: logical_esubst...
       by autosubst. }
     { have tyn':=ihn _ H3.
-      apply: sta0_pair1... } }
+      apply: logical0_pair1... } }
   { move=>Γ A B C m n s t tyC ihC tym ihm tyn ihn x st. inv st.
-    { have/sta0_sta_type tyA':=ihC _ H3.
-      move/sta0_sta_type in tyC.
-      move/sta0_sta_type in tym.
-      have//=tyCm:=sta_subst tyC tym.
-      have wf:=sta_type_wf tyC. inv wf.
-      have[s1[r[ord[tyA[tyB/sort_inj e]]]]]:=sta_sig0_inv H2; subst.
+    { have/logical0_logical_type tyA':=ihC _ H3.
+      move/logical0_logical_type in tyC.
+      move/logical0_logical_type in tym.
+      have//=tyCm:=logical_subst tyC tym.
+      have wf:=logical_type_wf tyC. inv wf.
+      have[s1[r[ord[tyA[tyB/sort_inj e]]]]]:=logical_sig0_inv H2; subst.
       have wkA':((Sig0 A B t).[ren (+2)] :: B :: A :: Γ) ⊢ A'.[ren (upren (+2))] : Sort s.
       { replace (Sort s) with (Sort s).[ren (upren (+2))] by eauto.
-        apply: sta_rename...
-        apply: sta_agree_ren_cons...
+        apply: logical_rename...
+        apply: logical_agree_ren_cons...
         replace (+2) with (id >>> (+1) >>> (+1)) by autosubst.
-        apply: sta_agree_ren_wk...
-        apply: sta_agree_ren_wk...
-        apply: sta_agree_ren_refl... }
+        apply: logical_agree_ren_wk...
+        apply: logical_agree_ren_wk...
+        apply: logical_agree_ren_refl... }
       have tyP:(B :: A :: Γ) ⊢ Pair0 (Var 1) (Var 0) t : (Sig0 A B t).[ren (+2)].
-      { apply: sta_pair0.
+      { apply: logical_pair0.
         { replace (Sig0 A.[ren (+2)] B.[up (ren (+2))] t)
           with (Sig0 A B t).[ren (+1)].[ren (+1)] by autosubst.
-          apply: sta_eweaken...
+          apply: logical_eweaken...
           instantiate (1 := Sort t)=>//.
-          apply: sta_eweaken... eauto. }
+          apply: logical_eweaken... eauto. }
         { replace A.[ren (+2)] with A.[ren (+1)].[ren (+1)] by autosubst.
           repeat constructor.
           econstructor... }
         { asimpl.
           repeat constructor.
           econstructor... } }
-      have{}xA':=sta_subst wkA' tyP. asimpl in xA'.
-      apply:sta0_conv.
-      apply: sta_conv_subst.
+      have{}xA':=logical_subst wkA' tyP. asimpl in xA'.
+      apply:logical0_conv.
+      apply: logical_conv_subst.
       apply: conv1i...
-      apply: sta0_letin0...
-      apply: sta0_conv.
-      apply: sta_conv_subst.
+      apply: logical0_letin0...
+      apply: logical0_conv.
+      apply: logical_conv_subst.
       apply: conv1...
       apply: tyn.
-      apply: sta_sta0_type...
+      apply: logical_logical0_type...
       eauto. }
-    { have/sta0_sta_type tym':=ihm _ H3.
-      move/sta0_sta_type in tyC.
-      move/sta0_sta_type in tym.
-      have//=tyCm:=sta_subst tyC tym.
-      apply: sta0_conv.
-      apply: sta_conv_beta.
+    { have/logical0_logical_type tym':=ihm _ H3.
+      move/logical0_logical_type in tyC.
+      move/logical0_logical_type in tym.
+      have//=tyCm:=logical_subst tyC tym.
+      apply: logical0_conv.
+      apply: logical_conv_beta.
       apply: conv1i...
-      apply: sta0_letin0...
+      apply: logical0_letin0...
       eauto... }
-    { have tyn':=ihn _ H3. apply: sta0_letin0... }
-    { move/sta0_sta_type in tyn.
-      move/sta0_sta_type in tym.
-      have[e[tym1 tym2]]:=sta_pair0_inv tym; subst.
-      apply: sta_sta0_type.
+    { have tyn':=ihn _ H3. apply: logical0_letin0... }
+    { move/logical0_logical_type in tyn.
+      move/logical0_logical_type in tym.
+      have[e[tym1 tym2]]:=logical_pair0_inv tym; subst.
+      apply: logical_logical0_type.
       replace C.[Pair0 m1 m2 t/]
         with C.[Pair0 (Var 1) (Var 0) t .: ren (+2)].[m2,m1/] by autosubst.
-      apply: sta_substitution...
+      apply: logical_substitution...
       repeat constructor...
       by asimpl. }
-    { move/sta0_sta_type in tym.
-      exfalso. apply: sta_pair1_sig0_false... } }
+    { move/logical0_logical_type in tym.
+      exfalso. apply: logical_pair1_sig0_false... } }
   { move=>Γ A B C m n s t tyC ihC tym ihm tyn ihn x st. inv st.
-    { have/sta0_sta_type tyA':=ihC _ H3.
-      move/sta0_sta_type in tyC.
-      move/sta0_sta_type in tym.
-      have//=tyCm:=sta_subst tyC tym.
-      have wf:=sta_type_wf tyC. inv wf.
-      have[s1[r[ord1[ord2[tyA[tyB/sort_inj e]]]]]]:=sta_sig1_inv H2; subst.
+    { have/logical0_logical_type tyA':=ihC _ H3.
+      move/logical0_logical_type in tyC.
+      move/logical0_logical_type in tym.
+      have//=tyCm:=logical_subst tyC tym.
+      have wf:=logical_type_wf tyC. inv wf.
+      have[s1[r[ord1[ord2[tyA[tyB/sort_inj e]]]]]]:=logical_sig1_inv H2; subst.
       have wkA':((Sig1 A B t).[ren (+2)] :: B :: A :: Γ) ⊢ A'.[ren (upren (+2))] : Sort s.
       { replace (Sort s) with (Sort s).[ren (upren (+2))] by eauto.
-        apply: sta_rename...
-        apply: sta_agree_ren_cons...
+        apply: logical_rename...
+        apply: logical_agree_ren_cons...
         replace (+2) with (id >>> (+1) >>> (+1)) by autosubst.
-        apply: sta_agree_ren_wk...
-        apply: sta_agree_ren_wk...
-        apply: sta_agree_ren_refl... }
+        apply: logical_agree_ren_wk...
+        apply: logical_agree_ren_wk...
+        apply: logical_agree_ren_refl... }
       have tyP:(B :: A :: Γ) ⊢ Pair1 (Var 1) (Var 0) t : (Sig1 A B t).[ren (+2)].
-      { apply: sta_pair1.
+      { apply: logical_pair1.
         { replace (Sig1 A.[ren (+2)] B.[up (ren (+2))] t)
           with (Sig1 A B t).[ren (+1)].[ren (+1)] by autosubst.
-          apply: sta_eweaken...
+          apply: logical_eweaken...
           instantiate (1 := Sort t)=>//.
-          apply: sta_eweaken... eauto. }
+          apply: logical_eweaken... eauto. }
         { replace A.[ren (+2)] with A.[ren (+1)].[ren (+1)] by autosubst.
           repeat constructor.
           econstructor... }
         { asimpl.
           repeat constructor.
           econstructor... } }
-      have{}xA':=sta_subst wkA' tyP. asimpl in xA'.
-      apply:sta0_conv.
-      apply: sta_conv_subst.
+      have{}xA':=logical_subst wkA' tyP. asimpl in xA'.
+      apply:logical0_conv.
+      apply: logical_conv_subst.
       apply: conv1i...
-      apply: sta0_letin1...
-      apply: sta0_conv.
-      apply: sta_conv_subst.
+      apply: logical0_letin1...
+      apply: logical0_conv.
+      apply: logical_conv_subst.
       apply: conv1...
       apply: tyn.
-      apply: sta_sta0_type...
+      apply: logical_logical0_type...
       eauto. }
-    { have/sta0_sta_type tym':=ihm _ H3.
-      move/sta0_sta_type in tyC.
-      move/sta0_sta_type in tym.
-      have//=tyCm:=sta_subst tyC tym.
-      apply: sta0_conv.
-      apply: sta_conv_beta.
+    { have/logical0_logical_type tym':=ihm _ H3.
+      move/logical0_logical_type in tyC.
+      move/logical0_logical_type in tym.
+      have//=tyCm:=logical_subst tyC tym.
+      apply: logical0_conv.
+      apply: logical_conv_beta.
       apply: conv1i...
-      apply: sta0_letin1...
+      apply: logical0_letin1...
       eauto... }
-    { have tyn':=ihn _ H3. apply: sta0_letin1... }
-    { move/sta0_sta_type in tym.
-      exfalso. apply: sta_pair0_sig1_false... }
-    { move/sta0_sta_type in tyn.
-      move/sta0_sta_type in tym.
-      have[e[tym1 tym2]]:=sta_pair1_inv tym; subst.
-      apply: sta_sta0_type.
+    { have tyn':=ihn _ H3. apply: logical0_letin1... }
+    { move/logical0_logical_type in tym.
+      exfalso. apply: logical_pair0_sig1_false... }
+    { move/logical0_logical_type in tyn.
+      move/logical0_logical_type in tym.
+      have[e[tym1 tym2]]:=logical_pair1_inv tym; subst.
+      apply: logical_logical0_type.
       replace C.[Pair1 m1 m2 t/]
         with C.[Pair1 (Var 1) (Var 0) t .: ren (+2)].[m2,m1/] by autosubst.
-      apply: sta_substitution...
+      apply: logical_substitution...
       repeat constructor...
       by asimpl. } }
   { move=>Γ A B s r t tyA ihA tyB ihB n st. inv st.
-    { have tyA':=ihA _ H3. apply: sta0_with... }
-    { have tyB':=ihB _ H3. apply: sta0_with... } }
+    { have tyA':=ihA _ H3. apply: logical0_with... }
+    { have tyB':=ihB _ H3. apply: logical0_with... } }
   { move=>Γ A B m n t tym ihm tyn ihn n0 st. inv st.
-    { have tym':=ihm _ H3. apply: sta0_apair... }
-    { have tyn':=ihn _ H3. apply: sta0_apair... } }
+    { have tym':=ihm _ H3. apply: logical0_apair... }
+    { have tyn':=ihn _ H3. apply: logical0_apair... } }
   { move=>Γ A B m t tym ihm n st. inv st.
-    { have tym':=ihm _ H0. apply: sta0_fst... }
-    { move/sta0_sta_type in tym.
-      have[_[tyn _]]:=sta_apair_inv tym... } }
+    { have tym':=ihm _ H0. apply: logical0_fst... }
+    { move/logical0_logical_type in tym.
+      have[_[tyn _]]:=logical_apair_inv tym... } }
   { move=>Γ A B m t tym ihm n st. inv st.
-    { have tym':=ihm _ H0. apply: sta0_snd... }
-    { move/sta0_sta_type in tym.
-      have[_[_ tyn]]:=sta_apair_inv tym... } }
+    { have tym':=ihm _ H0. apply: logical0_snd... }
+    { move/logical0_logical_type in tym.
+      have[_[_ tyn]]:=logical_apair_inv tym... } }
   { move=>Γ A m n s tyA ihA tym ihm tyn ihn n0 st. inv st.
     { have tyA':=ihA _ H3.
-      apply: sta0_id...
-      apply: sta0_conv.
+      apply: logical0_id...
+      apply: logical0_conv.
       apply: conv1...
       all: eauto.
-      apply: sta0_conv.
+      apply: logical0_conv.
       apply: conv1...
       all: eauto. }
-    { have tym':=ihm _ H3. apply: sta0_id... }
-    { have tyn':=ihn _ H3. apply: sta0_id... } }
+    { have tym':=ihm _ H3. apply: logical0_id... }
+    { have tyn':=ihn _ H3. apply: logical0_id... } }
   { move=>Γ A m tym ihm n st. inv st.
-    move/sta0_sta_type in tym.
-    have[s tyA]:=sta_valid tym.
+    move/logical0_logical_type in tym.
+    have[s tyA]:=logical_valid tym.
     have tym':=ihm _ H0.
-    apply: sta0_conv.
-    apply: sta_conv_id.
+    apply: logical0_conv.
+    apply: logical_conv_id.
     eauto.
     apply: conv1i...
     apply: conv1i...
-    apply: sta0_refl...
-    apply: sta0_id... }
+    apply: logical0_refl...
+    apply: logical0_id... }
   { move=>Γ A B H P m n s tyB ihB tyH ihH tyP ihP n0 st. inv st.
-    { have/sta0_sta_type tyA':=ihB _ H5.
-      move/sta0_sta_type in tyB.
-      move/sta0_sta_type in tyH.
-      move/sta0_sta_type in tyP.
-      have[r tyI]:=sta_valid tyP.
-      have[tym[tyn/sort_inj e]]:=sta_id_inv tyI; subst.
+    { have/logical0_logical_type tyA':=ihB _ H5.
+      move/logical0_logical_type in tyB.
+      move/logical0_logical_type in tyH.
+      move/logical0_logical_type in tyP.
+      have[r tyI]:=logical_valid tyP.
+      have[tym[tyn/sort_inj e]]:=logical_id_inv tyI; subst.
       have wkA':Γ ⊢ A'.[Refl m,m/] : Sort s.
       { replace (Sort s) with (Sort s).[Refl m,m/] by eauto.
-        apply: sta_substitution...
+        apply: logical_substitution...
         repeat constructor...
         all: asimpl...  }
       have wkB:Γ ⊢ B.[P,n/] : Sort s.
       { replace (Sort s) with (Sort s).[P,n/] by eauto.
-        apply: sta_substitution...
+        apply: logical_substitution...
         repeat constructor...
         all: asimpl... }
-      apply: sta0_conv.
-      apply: sta_conv_subst.
+      apply: logical0_conv.
+      apply: logical_conv_subst.
       apply: conv1i...
-      apply: sta0_rw...
-      apply: sta0_conv.
-      apply: sta_conv_subst.
+      apply: logical0_rw...
+      apply: logical0_conv.
+      apply: logical_conv_subst.
       apply: conv1...
       all: eauto. }
-    { have tyH':=ihH _ H5. apply: sta0_rw... }
-    { have/sta0_sta_type tyP':=ihP _ H5.
-      move/sta0_sta_type in tyB.
-      move/sta0_sta_type in tyH.
-      move/sta0_sta_type in tyP.
-      have[r tyI]:=sta_valid tyP.
-      have[tym[tyn/sort_inj e]]:=sta_id_inv tyI; subst.
+    { have tyH':=ihH _ H5. apply: logical0_rw... }
+    { have/logical0_logical_type tyP':=ihP _ H5.
+      move/logical0_logical_type in tyB.
+      move/logical0_logical_type in tyH.
+      move/logical0_logical_type in tyP.
+      have[r tyI]:=logical_valid tyP.
+      have[tym[tyn/sort_inj e]]:=logical_id_inv tyI; subst.
       have sc:sconv (P' .: n .: ids) (P .: n .: ids).
       { move=>[|]//=. apply: conv1i... }
       have wkB:Γ ⊢ B.[P,n/] : Sort s.
       { replace (Sort s) with (Sort s).[P,n/] by eauto.
-        apply: sta_substitution...
+        apply: logical_substitution...
         repeat constructor...
         all: asimpl... }
-      apply: sta0_conv.
-      apply: sta_conv_compat sc.
-      apply: sta0_rw...
+      apply: logical0_conv.
+      apply: logical_conv_compat sc.
+      apply: logical0_rw...
       eauto. }
-    { move/sta0_sta_type in tyB.
-      move/sta0_sta_type in tyH.
-      move/sta0_sta_type in tyP.
-      have[tym0[eq1 eq2]]:=sta_refl_inv tyP.
-      have[r tyI]:=sta_valid tyP.
-      have[tym[tyn/sort_inj e]]:=sta_id_inv tyI; subst.
+    { move/logical0_logical_type in tyB.
+      move/logical0_logical_type in tyH.
+      move/logical0_logical_type in tyP.
+      have[tym0[eq1 eq2]]:=logical_refl_inv tyP.
+      have[r tyI]:=logical_valid tyP.
+      have[tym[tyn/sort_inj e]]:=logical_id_inv tyI; subst.
       have sc:sconv (Refl m .: m .: ids) (Refl m0 .: n .: ids).
       { move=>[|[|]]//=.
-        apply: sta_conv_refl. apply: conv_sym...
+        apply: logical_conv_refl. apply: conv_sym...
         apply: conv_trans. apply: conv_sym... eauto. }
       have wkB:Γ ⊢ B.[Refl m0,n/] : Sort s.
       { replace (Sort s) with (Sort s).[Refl m0,n/] by eauto.
-        apply: sta_substitution...
+        apply: logical_substitution...
         repeat constructor...
         all: asimpl... }
-      apply: sta0_conv.
-      apply: sta_conv_compat sc.
+      apply: logical0_conv.
+      apply: logical_conv_compat sc.
       all: eauto. } }
 Qed.
 
-Corollary sta_rd Γ m n A :
+(* Iterated steps preserve logical typing. *)
+Corollary logical_rd Γ m n A :
   Γ ⊢ m : A -> m ~>* n -> Γ ⊢ n : A.
 Proof with eauto.
   move=>ty rd. elim: rd Γ A ty=>{n}...
   move=>n z rd ih st Γ A tym.
   have tyn:=ih _ _ tym.
-  apply: sta_sr...
+  apply: logical_sr...
 Qed.
