coq/theories/logical_valid.v
@@ -1,46 +1,52 @@
+(* This file presents the type validity theorem of the logical level.
+   Additional inversion lemmas can be proven using type validity *)
+
 From mathcomp Require Import ssreflect ssrbool eqtype ssrnat seq.
 From Coq Require Import ssrfun Classical Utf8.
-Require Export AutosubstSsr ARS sta_inv.
+Require Export AutosubstSsr ARS logical_inv.
 
 Set Implicit Arguments.
 Unset Strict Implicit.
 Unset Printing Implicit Defensive.
 
-Theorem sta_valid Γ m A : Γ ⊢ m : A -> exists s, Γ ⊢ A : Sort s.
-Proof with eauto using sta_type.
+(* Theorem 2 (Type Validity) *)
+Theorem logical_valid Γ m A : Γ ⊢ m : A -> exists s, Γ ⊢ A : Sort s.
+Proof with eauto using logical_type.
   move=>ty. elim: ty=>{Γ m A}...
   { move=>Γ x A wf hs.
-    apply: sta_wf_ok... }
+    apply: logical_wf_ok... }
   { move=>Γ A B m s tym [t tyB].
-    have wf:=sta_type_wf tyB.
+    have wf:=logical_type_wf tyB.
     exists s. inv wf... }
   { move=>Γ A B m s tym [t tyB].
-    have wf:=sta_type_wf tyB.
+    have wf:=logical_type_wf tyB.
     exists s. inv wf... }
   { move=>Γ A B m n s
-      tym[s0/sta_pi0_inv[t[tyB/sort_inj e1]]]tyn _; subst.
-    exists t. apply: sta_esubst...
+      tym[s0/logical_pi0_inv[t[tyB/sort_inj e1]]]tyn _; subst.
+    exists t. apply: logical_esubst...
     by autosubst. }
   { move=>Γ A B m n s
-      tym[s0/sta_pi1_inv[t[tyB/sort_inj e1]]]tyn _; subst.
-    exists t. apply: sta_esubst...
+      tym[s0/logical_pi1_inv[t[tyB/sort_inj e1]]]tyn _; subst.
+    exists t. apply: logical_esubst...
     by autosubst. }
   { move=>Γ A B C m n s t tyC _ tym _ _ _.
-    have//={}tyC:=sta_subst tyC tym. exists s... }
+    have//={}tyC:=logical_subst tyC tym. exists s... }
   { move=>Γ A B C m n s t tyC _ tym _ _ _.
-    have//={}tyC:=sta_subst tyC tym. exists s... }
+    have//={}tyC:=logical_subst tyC tym. exists s... }
   { move=>Γ A B m n t _[s tyA]_[r tyB]. exists t... }
-  { move=>Γ A B m t _[s/sta_with_inv[r[_[tyA _]]]]. exists r... }
-  { move=>Γ A B m t _[s/sta_with_inv[_[r[_[tyB _]]]]]. exists r... }
+  { move=>Γ A B m t _[s/logical_with_inv[r[_[tyA _]]]]. exists r... }
+  { move=>Γ A B m t _[s/logical_with_inv[_[r[_[tyB _]]]]]. exists r... }
   { move=>Γ A m tym[s tyA]. exists U... }
   { move=>Γ A B H P m n s tyB _ tyH _ tyP[r tyI].
-    have[tym[tyn _]]:=sta_id_inv tyI. exists s.
+    have[tym[tyn _]]:=logical_id_inv tyI. exists s.
     replace (Sort s) with (Sort s).[P,n/] by autosubst.
-    apply: sta_substitution...
+    apply: logical_substitution...
     repeat constructor; asimpl... }
 Qed.
 
-Lemma sta_lam0_invX Γ A1 A2 B C m s1 s2 t :
+(* More inversion lemmas are provable with Type Validity. *)
+
+Lemma logical_lam0_invX Γ A1 A2 B C m s1 s2 t :
   Γ ⊢ Lam0 A1 m s1 : C ->
   C === Pi0 A2 B s2 ->
   (A2 :: Γ) ⊢ B : Sort t ->
@@ -50,20 +56,20 @@ Proof with eauto.
   elim: tyL A1 A2 B m s1 s2 t e=>//{Γ C n}.
   { move=>Γ A B m s tym _ A1 A2 B0 m0
       s1 s2 t[e1 e2 e3]/pi0_inj[eq1[eq2 e4]]tyB0; subst.
-    have wf:=sta_type_wf tym. inv wf.
-    have wf:=sta_type_wf tyB0. inv wf.
-    apply: sta_ctx_conv.
+    have wf:=logical_type_wf tym. inv wf.
+    have wf:=logical_type_wf tyB0. inv wf.
+    apply: logical_ctx_conv.
     apply: conv_sym...
     exact: H4.
-    apply: sta_conv...
-    apply: sta_ctx_conv... }
+    apply: logical_conv...
+    apply: logical_ctx_conv... }
   { move=>Γ A B m s eq1 tym ihm tyB ihB A1 A2 B0 m0
       s1 s2 t e eq2 tyB0; subst.
     apply: ihm...
     apply: conv_trans... }
 Qed.
 
-Lemma sta_lam1_invX Γ A1 A2 B C m s1 s2 t :
+Lemma logical_lam1_invX Γ A1 A2 B C m s1 s2 t :
   Γ ⊢ Lam1 A1 m s1 : C ->
   C === Pi1 A2 B s2 ->
   (A2 :: Γ) ⊢ B : Sort t ->
@@ -73,36 +79,36 @@ Proof with eauto.
   elim: tyL A1 A2 B m s1 s2 t e=>//{Γ C n}.
   { move=>Γ A B m s tym _ A1 A2 B0 m0
       s1 s2 t[e1 e2 e3]/pi1_inj[eq1[eq2 e4]]tyB0; subst.
-    have wf:=sta_type_wf tym. inv wf.
-    have wf:=sta_type_wf tyB0. inv wf.
-    apply: sta_ctx_conv.
+    have wf:=logical_type_wf tym. inv wf.
+    have wf:=logical_type_wf tyB0. inv wf.
+    apply: logical_ctx_conv.
     apply: conv_sym...
     exact: H4.
-    apply: sta_conv...
-    apply: sta_ctx_conv... }
+    apply: logical_conv...
+    apply: logical_ctx_conv... }
   { move=>Γ A B m s eq1 tym ihm tyB ihB A1 A2 B0 m0
       s1 s2 t e eq2 tyB0; subst.
     apply: ihm...
     apply: conv_trans... }
 Qed.
 
-Lemma sta_lam0_inv Γ m A1 A2 B s1 s2 :
+Lemma logical_lam0_inv Γ m A1 A2 B s1 s2 :
   Γ ⊢ Lam0 A2 m s2 : Pi0 A1 B s1 -> (A1 :: Γ) ⊢ m : B.
 Proof with eauto.
   move=>ty.
-  have[t/sta_pi0_inv[r[tyB _]]]:=sta_valid ty.
-  apply: sta_lam0_invX...
+  have[t/logical_pi0_inv[r[tyB _]]]:=logical_valid ty.
+  apply: logical_lam0_invX...
 Qed.
 
-Lemma sta_lam1_inv Γ m A1 A2 B s1 s2 :
+Lemma logical_lam1_inv Γ m A1 A2 B s1 s2 :
   Γ ⊢ Lam1 A2 m s2 : Pi1 A1 B s1 -> (A1 :: Γ) ⊢ m : B.
 Proof with eauto.
   move=>ty.
-  have[t/sta_pi1_inv[r[tyB _]]]:=sta_valid ty.
-  apply: sta_lam1_invX...
+  have[t/logical_pi1_inv[r[tyB _]]]:=logical_valid ty.
+  apply: logical_lam1_invX...
 Qed.
 
-Lemma sta_pair0_invX Γ m n s C :
+Lemma logical_pair0_invX Γ m n s C :
   Γ ⊢ Pair0 m n s : C ->
   forall A B r t,
     C === Sig0 A B r ->
@@ -113,20 +119,20 @@ Proof with eauto.
   elim: ty m n s e=>//{Γ C x}.
   { move=>Γ A B m n t ty1 _ tym _ tyn _ m0 n0 s[e1 e2 e3]A0 B0 r t0
       /sig0_inj[e4[e5 e6]]ty2; subst.
-    have[s[r0[ord[tyA0[tyB0/sort_inj e]]]]]:=sta_sig0_inv ty2; subst.
-    have tym0:Γ ⊢ m : A0 by apply: sta_conv; eauto.
+    have[s[r0[ord[tyA0[tyB0/sort_inj e]]]]]:=logical_sig0_inv ty2; subst.
+    have tym0:Γ ⊢ m : A0 by apply: logical_conv; eauto.
     repeat split...
-    apply: sta_conv.
-    apply: sta_conv_subst.
+    apply: logical_conv.
+    apply: logical_conv_subst.
     all: eauto.
-    apply: sta_esubst...
+    apply: logical_esubst...
     by autosubst. }
   { move=>Γ A B m s eq tym ihm _ _ m0 n s0 e A0 B0 r t eq' ty.
     apply: ihm...
     apply: conv_trans... }
 Qed.
 
-Lemma sta_pair1_invX Γ m n s C :
+Lemma logical_pair1_invX Γ m n s C :
   Γ ⊢ Pair1 m n s : C ->
   forall A B r t,
     C === Sig1 A B r ->
@@ -137,38 +143,38 @@ Proof with eauto.
   elim: ty m n s e=>//{Γ C x}.
   { move=>Γ A B m n t ty1 _ tym _ tyn _ m0 n0 s[e1 e2 e3]A0 B0 r t0
       /sig1_inj[e4[e5 e6]]ty2; subst.
-    have[s[r0[ord1[ord2[tyA0[tyB0/sort_inj e]]]]]]:=sta_sig1_inv ty2; subst.
-    have tym0:Γ ⊢ m : A0 by apply: sta_conv; eauto.
+    have[s[r0[ord1[ord2[tyA0[tyB0/sort_inj e]]]]]]:=logical_sig1_inv ty2; subst.
+    have tym0:Γ ⊢ m : A0 by apply: logical_conv; eauto.
     repeat split...
-    apply: sta_conv.
-    apply: sta_conv_subst.
+    apply: logical_conv.
+    apply: logical_conv_subst.
     all: eauto.
-    apply: sta_esubst...
+    apply: logical_esubst...
     by autosubst. }
   { move=>Γ A B m s eq tym ihm _ _ m0 n s0 e A0 B0 r t eq' ty.
     apply: ihm...
     apply: conv_trans... }
 Qed.
 
-Lemma sta_pair0_inv Γ A B m n s r :
+Lemma logical_pair0_inv Γ A B m n s r :
   Γ ⊢ Pair0 m n s : Sig0 A B r ->
   s = r /\ Γ ⊢ m : A /\ Γ ⊢ n : B.[m/].
 Proof with eauto.
   move=>ty.
-  have[t tyS]:=sta_valid ty.
-  apply: sta_pair0_invX...
+  have[t tyS]:=logical_valid ty.
+  apply: logical_pair0_invX...
 Qed.
 
-Lemma sta_pair1_inv Γ A B m n s r :
+Lemma logical_pair1_inv Γ A B m n s r :
   Γ ⊢ Pair1 m n s : Sig1 A B r ->
   s = r /\ Γ ⊢ m : A /\ Γ ⊢ n : B.[m/].
 Proof with eauto.
   move=>ty.
-  have[t tyS]:=sta_valid ty.
-  apply: sta_pair1_invX...
+  have[t tyS]:=logical_valid ty.
+  apply: logical_pair1_invX...
 Qed.
 
-Lemma sta_apair_invX Γ m n s C :
+Lemma logical_apair_invX Γ m n s C :
   Γ ⊢ APair m n s : C ->
   forall A B r t,
     C === With A B r ->
@@ -179,25 +185,25 @@ Proof with eauto.
   elim: ty m n s e=>//{Γ C x}.
   { move=>Γ A B m n t tym ihm tyn ihn m0 n0 s[e1 e2 e3]A0 B0 r t0
       /with_inj[e4[e5 e6]]ty; subst.
-    have[s[r0[tyA0[tyB0 _]]]]:=sta_with_inv ty.
+    have[s[r0[tyA0[tyB0 _]]]]:=logical_with_inv ty.
     repeat split...
-    apply: sta_conv...
-    apply: sta_conv... }
+    apply: logical_conv...
+    apply: logical_conv... }
   { move=>Γ A B m s eq1 tym ihm _ _ m0 n s0 e A0 B0 r t eq' tyw; subst.
     apply: ihm...
     apply: conv_trans... }
 Qed.
 
-Lemma sta_apair_inv Γ m n A B s r :
+Lemma logical_apair_inv Γ m n A B s r :
   Γ ⊢ APair m n s : With A B r ->
   s = r /\ Γ ⊢ m : A /\ Γ ⊢ n : B.
 Proof with eauto.
   move=>ty.
-  have[t tyW]:=sta_valid ty.
-  apply: sta_apair_invX...
+  have[t tyW]:=logical_valid ty.
+  apply: logical_apair_invX...
 Qed.
 
-Lemma sta_refl_invX Γ n C :
+Lemma logical_refl_invX Γ n C :
   Γ ⊢ Refl n : C ->
   forall A m1 m2 s,
     C === Id A m1 m2 ->
@@ -207,19 +213,19 @@ Proof with eauto.
   move e:(Refl n)=>x ty.
   elim: ty n e=>//{Γ x C}.
   { move=>Γ A m tym ihm n[e1]A0 m1 m2 s/id_inj[e2[e3 e4]]tyI; subst.
-    have[tym1 _]:=sta_id_inv tyI.
-    have[r tyA0]:=sta_valid tym1.
+    have[tym1 _]:=logical_id_inv tyI.
+    have[r tyA0]:=logical_valid tym1.
     repeat split...
-    apply: sta_conv... }
+    apply: logical_conv... }
   { move=>Γ A B m s eqw tym ihm _ _ n e A0 m1 m2 s0 eq' tyI.
     apply: ihm...
     apply: conv_trans... }
 Qed.
 
-Lemma sta_refl_inv Γ A m1 m2 n :
+Lemma logical_refl_inv Γ A m1 m2 n :
   Γ ⊢ Refl n : Id A m1 m2 -> Γ ⊢ n : A /\ n === m1 /\ n === m2.
 Proof with eauto.
   move=>ty.
-  have[s tyI]:=sta_valid ty.
-  apply: sta_refl_invX...
+  have[s tyI]:=logical_valid ty.
+  apply: logical_refl_invX...
 Qed.
